\documentclass{article}

\input{D:/Notes/others/myHeadings.tex}

\title{HW3}
\author{Yuanxing Cheng, A20453410, MMAE-501-f22}

\begin{document}

\maketitle

\section*{1}


\begin{myleftlinebox}
    Solve the system 
    \begin{align*}
        \frac{\dif x_1}{\dif t} = x_1 + 2 x_2\\
        \frac{\dif x_2}{\dif t} = 2 x_1 + x_2
    \end{align*}
    subject to initial condition \(x_1(0) = 1\), \(x_2(0) = 3\).
    \tcblower
    Write the equation as \(\frac{\dif X}{\dif t} = AX\) where \(X = [x_1,x_2]^\top\) and \(A = \begin{bmatrix}
        1 & 2 \\
        2 & 1
    \end{bmatrix}\)
    For matrix \(A\) we find its eigenvalue and eigenvector pairs. We first solve \(\det (\lambda I-A) = (\lambda-1)^2-(-2)^2 = (\lambda-3)(\lambda+1)=0\) so \(\lambda_1 = 3\) and \(\lambda_2 = -1\). Their corresponding eigenvectors are obtained by solving \(\lambda_i I-A=0\) which gives \(x_1 = [1, 1]^\top\) and \(x_2 = [1,-1]^\top\). So we write the solution in the matrix form as

    \begin{equation*}
        X(t) = [x_1,x_2][c_1 e^{\lambda_1 t}, c_2 e^{\lambda_2 t}]^\top = \begin{bmatrix}
            1 & 1\\
            1 & -1
        \end{bmatrix}\begin{bmatrix}
            c_1 e^{3 t}\\
            c_2 e^{-t}
        \end{bmatrix}
    \end{equation*}
    plug in intial conditions we have \(X(0) = [1,3]^\top = \begin{bmatrix}
        1 & 1\\
        1 & -1
    \end{bmatrix}[c_1,c_2]^\top\), then solve this we have \([c_1,c_2]=[2,-1]\). The final solution is then 
    \begin{align*}
        x_1(t) &= 2 e^{3t} - e^{-t}\\
        x_2(t) &= 2 e^{3t} + e^{-t}
    \end{align*}
\end{myleftlinebox}

\section*{2}
\begin{myleftlinebox}
    Verify by direct calculation that the matrix \(A = \begin{bmatrix}
        -2 & -3 & -1\\
        1 & 2 & 1\\
        3 & 3 & 2
    \end{bmatrix}\) satisfies the Cayleyâ€“Hamilton theorem.
    \tcblower
    \begin{equation*}
        \begin{split}
            p_A(\lambda) &= (\lambda+2)(\lambda-2)(\lambda-2)+9+3+3(\lambda-2)+3(\lambda-2)-3(\lambda+2)\\
            &= \lambda^3-2\lambda^2-4\lambda+8+12+3\lambda-18\\
            &= \lambda^3-2\lambda^2-\lambda+2\\
        \end{split}
    \end{equation*}
    Next we plug in \(\lambda=A\), we obtain the following:
    \begin{equation*}
        \begin{split}
            p_A(A) &= \begin{bmatrix}
                -8 & -9 & -7 \\
                7 & 8 & 7\\
                9 & 9 & 8
            \end{bmatrix}-2\begin{bmatrix}
                -2 & -3 & -3\\
                3 & 4 & 3\\
                3 & 3 & 4
            \end{bmatrix}-\begin{bmatrix}
                -2 & -3 & -1\\
                1 & 2 & 1\\
                3 & 3 & 2
            \end{bmatrix}+\begin{bmatrix}
                2 & 0 & 0\\
                0 & 2 & 0\\
                0 & 0 & 2
            \end{bmatrix}\\
            &=\begin{bmatrix}
                -8+4+2+2 & -9+6+3+0 & -7+6+1+0\\
                7-6-1+0 & 8-8-2+2 & 7-6-1+0\\
                9-6-3-0 & 9-6-3-0 & 8-8-2+2    
            \end{bmatrix} = 0
        \end{split}
    \end{equation*}
\end{myleftlinebox}

\section*{3}
\begin{myleftlinebox}
    Determine the general solution of the following system of equations by diagonalization
    \begin{align*}
        \dot x_1 &= -10 x_1-18 x_2+t\\
        \dot x_2 &= 6 x_1 +11 x_2+3
    \end{align*}
    \tcblower
    We first rewrite the original system as \(\dot X(t) = AX(t)+f(t)\) where \(A = \begin{bmatrix}
        -10 & -18\\
        6 & 11
    \end{bmatrix}\) and \(f(t) = [t,3]^\top\). Use the same way, we first get the eigenvalues of matrix \(A\), \(\lambda_1 = 2\) and \(\lambda_2 = -1\), and corresponding eigenvectors are \([3,-2]^\top\) and \([2,-1]^\top\) so we have the diagonalization \(A = B\Lambda B^{-1}\) where \(\Lambda = \begin{bmatrix}
        2 & 0 \\
        0 & -1
    \end{bmatrix}\) and \(B = \begin{bmatrix}
        3 & 2\\
        -2 & -1
    \end{bmatrix}\). We can then let \(X = BY\) and left multiply \(B^{-1}\) on both side and obtain the following equation.
    \begin{equation*}
        \dot Y(t) = \Lambda Y(t)+B^{-1}f(t)
    \end{equation*}
    We first solve the homogenous equation \(y_1(t) = c_1 e^{2t}\) and \(y_2(t)=c_2 e^{-t}\); then guess the particular solution. 
    \begin{equation*}
        B^{-1}f(t) = [-t-6,2t+9]^\top\implies y_1(t) = \frac{1}{2}t+\frac{13}{4}, y_2(t) = 2t+7
    \end{equation*}
    We can then combine these two results and obtain the final solution for \(Y\) as
    \begin{equation*}
        y_1(t) = c_1 e^{2t} +\frac{1}{2}t+\frac{13}{4},y_2(t) = c_2 e^{-t}+ 2t+7
    \end{equation*}
    So that
    \begin{equation*}
        x_1(t) = 3y_1(t)+2y_2(t)= 3c_1 e^{2t}+2c_2 e^{-t} +\frac{11}{2}t+\frac{95}{4}, x_2(t) = -2y_1(t)-y_2(t) = -2c_1 e^{2t}-c_2 e^{-t} -3t-\frac{27}{2}
    \end{equation*}
\end{myleftlinebox}

\section*{4}
\begin{myleftlinebox}
    Determine the general solution of the following system of equations by diagonalization
    \begin{equation*}
        \begin{split}
            \dot x_1 &= -2x_1+2x_2+2x_3+\sin t\\
            \dot x_2 &= -x_2 + 3\\
            \dot x_3 &= -2x_1+4 x_2 + 3x_3
        \end{split}
    \end{equation*}
    \tcblower
    Similarly, we write \(\dot X = AX+f\) where \(A = \begin{bmatrix}
        -2 & 2 & 2\\
        0 & -1 & 0\\
        -2 & 4 & 3
    \end{bmatrix}\) and \(f=[\sin t,3,0]^\top\). We first find \(A\)'s eigenvalues \(\lambda_1 = 2\) and \(\lambda_2 = -1\), and corresponding eigenvectors \([1,0,2]^\top\), \([2,0,1]^\top\) and \([2,1,0]^\top\), so we have the diagonalization \(A = B\Lambda B^{-1}\) where \(\Lambda=\begin{bmatrix}
        2 & 0 & 0\\
        0 & -1 & 0\\
        0 & 0 & -1
    \end{bmatrix}\) and \(B = \begin{bmatrix}
        1 & 2 & 2\\
        0 & 1 & 0\\
        2 & 0 & 1
    \end{bmatrix}\). We then let \(X = BY\) and left multiply \(B^{-1}=\frac{1}{3}\begin{bmatrix}
        -1 & 2 & 2\\
        0 & 3 & 0\\
        2 & -4 & -1
    \end{bmatrix}\) and this gives \(\dot Y(t) = \Lambda Y(t) + B^{-1} f(t)\). So that \(y_1(t) = c_1 e^{2t}, y_{2,3}(t) = c_{2,3} e^{-t}\). Then we guess the particular solution using undetermined coefficients.
    \begin{equation*}
        \begin{split}
            C \cos t-D\sin t+E &= 2  C\sin t+2D\cos t+2E t+2F+\frac{1}{3}\Pare{-\sin t+6}\\
            \implies y_1(t) &= \frac{2}{15}\sin t+\frac{1}{15}\cos t-1\\
            C \cos t-D\sin t+E &= -C\sin t-D\cos t-Et-F+\frac{1}{3}(3*3)\\
            \implies y_2(t) &= 3\\
            C \cos t-D\sin t+E &=-C\sin t-D\cos t-Et-F+\frac{1}{3}\Pare{2\sin t-12}\\
            \implies y_3(t) &= \frac{1}{3}\sin t-\frac{1}{3}\cos t-4
        \end{split}
    \end{equation*}
    Then the general solution for \(Y\) is
    \begin{align*}
        y_1(t) &= c_1 e^{2t}+\frac{2}{15}\sin t+\frac{1}{15}\cos t-1\\
        y_2(t) &= c_2 e^{-t}+3\\
        y_3(t) &= c_3 e^{-t}+\frac{1}{3}\sin t-\frac{1}{3}\cos t-4
    \end{align*}
    And finally the general solution for \(X\) is 
    \begin{align*}
        x_1(t) &= y_1(t)+2y_2(t)+2y_3(t)\\
        &= c_1 e^{2t}+2(c_2+c_3)e^{-t}+\frac{4}{5}\sin t-\frac{3}{5}\cos t-3\\
        x_2(t) &= y_2(t)\\
        &= c_2 e^{-t}+3\\
        x_3(t) &= 2y_1(t)+y_3(t)\\
        &= 2c_1 e^{2t}+c_3 e^{-t}+\frac{3}{5}\sin t-\frac{1}{5}\cos t-6
    \end{align*}
\end{myleftlinebox}

\section*{5}
\begin{myleftlinebox}
    Determine the singular value decomposition of the matrix \(\begin{bmatrix}
        0 & 1 & 1\\
        \sqrt{2} & 2 & 0\\
        0 & 1 & 1
    \end{bmatrix}\). Compare the singular values and singular vectors of \(A\) to its eigenvalues and eigenvectors.
    \tcblower
    To find the singular values, we find the eigenvalues of \(AA^\top=\begin{bmatrix}
        2 & 2 & 2\\
        2 & 6 & 2\\
        2 & 2 & 2
    \end{bmatrix}\) which are \(8,2,0\) and corresponding eigenvectors are \([1,2,1]^\top,[1,-1,1]^\top,[-1,0,1]^\top\). So that \(U=\begin{bmatrix}
        1/\sqrt 6 & 1/\sqrt 3 & -1/\sqrt 2\\
        2/\sqrt 6 & -1/\sqrt 3 & 0\\
        1/\sqrt 6 & 1/\sqrt 3 & 1/\sqrt 2
    \end{bmatrix}\). Then \(v_1 = \frac{1}{\sqrt 8} A^\top u_1 = [\sqrt 6/6,\sqrt 3/2,\sqrt 3/6]^\top\), similarly, \(v_2 = [-\sqrt 3/3,0,\sqrt 6/3]^\top\), and for \(v_3\), just make \(v\)s an orthonormal basis. From \(v_2\),  we choose \(v_3 = [\sqrt 2,\eta, 1]\), then since \(v_1v_3=0\), we see \(\eta=-1\), after normalization, we obtain \(V = \begin{bmatrix}
        \sqrt6/6 & -\sqrt 3/3 & \sqrt 2/2\\
        \sqrt3/2 & 0 & -1/2\\
        \sqrt3/6 & \sqrt6/3 & 1/2
    \end{bmatrix}\). So that \(A = U\Sigma V^\top\) where \(\Sigma=\begin{bmatrix}
        2\sqrt 2 & 0 & 0\\\
        0 & \sqrt 2 & 0\\
        0 &0 & 0
    \end{bmatrix}\).
    
    Next we compare above with its eigenvalues and eigenvectors. We first obtain its characteristic polynomial as \(\lambda^3-3\lambda^2+(2-\sqrt 2)\lambda\) so \(\lambda_1=0\), \(\lambda_{2,3} = \frac{3\pm \sqrt{1+4\sqrt 2}}{2}\) and corresponding eigenvectors are \([\sqrt 2,-1,1]^\top\), \([1,\frac{1\pm \sqrt{1+4\sqrt 2}}{2},1]^\top\). They aren't very related.
\end{myleftlinebox}

\section*{6}

\begin{myleftlinebox}
    Consider the matrix \(\begin{bmatrix}
        1 & 0 & 1 & 0 & 1 & 0 & 1\\
        0 & 1 & 0 & 1 & 0 & 1 & 0
    \end{bmatrix}\) compute the left singular vectors and singular values of \(A\); then using the result find the first two right singular vectors of \(A\).
    \tcblower
    For the left singular values, we first compute \(AA^\top=\begin{bmatrix}
        4 & 0\\
        0 & 3
    \end{bmatrix}\) so matrix \(A\) has singular value \(\sqrt 4=2\), \( \sqrt 3\). And the singular vectors are the eigenvectors of \(AA^\top\) which are \(u_1=[1,0]^\top\) and \(u_2=[0,1]^\top\). 

    The first 2 right singular values can be found using the formula. \(v_1 = \frac{1}{2}A^\top u_1 = \frac{1}{2}[1,0,1,0,1,0,1]^\top\) and \(v_2 = \frac{1}{\sqrt 3}A^\top u_2 = \frac{1}{\sqrt 3}[0,1,0,1,0,1,0]^\top\).
\end{myleftlinebox}

%\newpage

%\bibliographystyle{acm}
%\bibliography{D:/Papers.bib}

%\newpage
%\appendix
%\section{Appendix}

\end{document}