\documentclass{article}
\usepackage[utf8]{inputenc}
\usepackage{graphicx}

\usepackage{amsthm, amsmath, amssymb, amsfonts, epsfig}
\usepackage{algorithm, algpseudocode}
\usepackage{algcompatible}
\input{../others/myHeadings.tex}
\usetikzlibrary{angles,quotes}

\title{Trigonometric Functions Review}
\author{Yuanxing Cheng}

\begin{document}

\maketitle

\section{Basics}
\begin{myleftlinebox}
    radian and degree
    \tcblower
    They are the unit of angle. And the standard unit is radian.
    \begin{itemize}
        \item $1$ radian is defined as the angle subtended from the center of a circle which intercepts an arc equal in length to the radius of the circle. 
        \item $360$ degree is one complete revolution.
    \end{itemize}
    Using radian measure, we have the relation, $s=\theta r$.
	\begin{center}
		\begin{tikzpicture}[
			my angle/.style = {
				draw, angle radius=7mm, 
				angle eccentricity=1.1, 
				right, inner sep=1pt,
				font=\footnotesize
				}
			]
			\coordinate (O) at (0,0);
			\coordinate (A) at (2,0);
			\coordinate (B) at (60:2);
			\coordinate (s) at (30:2);
			\draw (O) node[anchor=east,align=center] {$O$};
			\draw (O) circle (2);
			\draw (A) node[anchor=west,align=center] {$A$};
			\draw (B) node[xshift=0.3cm, yshift=0.2cm,align=center] {$B$};
			\draw (s) node[xshift=0.2cm, yshift=0.2cm,align=center] {$s$};
			\draw (O) -- (A)node[midway, below]{$r$, radius};
			\draw (O) -- (B);
			\pic[my angle,"$\theta$"] {angle = A--O--B};
		\end{tikzpicture}
	\end{center}
\end{myleftlinebox}

\begin{myleftlinebox}
	$\pi$
	\tcblower
	$\pi$ is defined as the ratio of a circle's circumference $C$ to its diameter $d$. So $C=\pi d=2\pi r$. A right angle is $\pi/2=90$ degree.
\end{myleftlinebox}

\begin{myleftlinebox}
	trigonometric function
	\tcblower
	Given a right triangle, an angle $x$ in radian measure. For this angle $x$, define the opposite side to be the side opposite to $x$, with length $a$, define the adjacent side to be the side between $x$ and the right angle, with length $b$, and the hypotenuse side to be the side opposite to the right angle, with length $c$, then
	
	$\sin(x) = a/c$, $\cos(x)=b/c$, and $\tan(x) = a/b$; then $\csc(x)=1/\sin(x)$, $\sec(x)=1/\cos(x)$ and $\cot(x)=1/	\tan(x)$.
	\begin{center}
		\begin{tikzpicture}[
			my angle/.style = {
				draw, angle radius=7mm, 
				angle eccentricity=1.1, 
				right, inner sep=1pt,
				font=\footnotesize
				}
			]
			\coordinate (a) at (0,0);
			\coordinate (c) at (4,0);
			\coordinate (b) at (4,2);
			\draw (a) -- (c)node[midway, below]{$b$, adjacent};
			\draw (b) -- (c)node[midway,right]{$a$, opposite};
			\draw (b) -- (a)node[midway,left, above,rotate=26.5]{$c$, hypotenuse}; % Triangle.
			\draw (a) node[anchor=east,align=center] {$A$};
			\draw (b) node[anchor=west,align=center] {$B$};
			\draw (c) node[anchor=west]{$C$};
			\draw pic[draw, angle radius=3mm] {right angle=a--c--b};
			\pic[my angle,"$x$"] {angle = c--a--b};
		\end{tikzpicture}
	\end{center}
\end{myleftlinebox}


\section{Conclusions}

\begin{myleftlinebox}
	area of circle
	\tcblower
	Using limit and squeeze theorem, we separate the area of a circle into $n$ number of annulus. Now the area of circle with radius $r$, $A$ satisfies the following:
	\[\sum_{i=0}^{n-1} \frac{r}{n}\Pare{2\pi \frac{r(i+1)}{n}}>A>\sum_{i=0}^{n-1} \frac{r}{n}\Pare{2\pi \frac{ri}{n}}\]
	\begin{center}
		\begin{tikzpicture}[scale=0.8]
			\coordinate (O) at (0,0);
			\coordinate (A) at (2,0);
			\coordinate (B) at (2.5,0);
			\coordinate (C) at (30:2);
			\coordinate (D) at (30:2.5);
			\draw (O) circle (2);
			\draw (O) circle (2.5);
			\draw (A) arc (0:30:2)node[midway,left]{$2\pi r_i$};
			\draw (B) arc (0:30:2.5)node[midway,right]{$2\pi r_{i+i}$};
			\draw (A) -- (B)node[midway, below]{$\frac{r}{n}$};
		\end{tikzpicture}
	\end{center}
	Above inequality is reduced to 
	\[\pi r^2 \frac{n+1}{n}>A>\pi r^2 \frac{n-1}{n}\]
	Then by squeeze theorem (for series not functions), $\lim_{n\to\infty} A = A=\pi r^2$.

	Similar idea can be used to find the area of a sector. For a sector of radius $r$ and angle $\theta$, its area is $\frac{1}{2}\theta r^2$. A linear function of $\theta$.

	We can also plug in the formula for arc length $s=\theta r$ and above becomes $\frac{1}{2} \theta s$, which is quite similar to the one for triangle.
\end{myleftlinebox}


\begin{myleftlinebox}
	Pythagorean Theorem
	\tcblower
	\begin{theorem}
		In any right triangle with sides of lengths $a$ and $b$, and hypotenuse of length $c$, we have $a^2+b^2=c^2$.
	\end{theorem}
	\begin{proof}
		We can put four triangles of the same size into the following square.

		\begin{center}
			\begin{tikzpicture}
				\coordinate (A) at (-2,-2);
				\coordinate (B) at (2,-2);
				\coordinate (C) at (2,2);
				\coordinate (D) at (-2,2);
				\coordinate (O) at (0,0);
				\coordinate (E) at (-1,-2);
				\coordinate (F) at (2,-1);
				\coordinate (G) at (1,2);
				\coordinate (H) at (-2,1);
				\draw (A) node[below]{$A$};
				\draw (E) node[below]{$E$};
				\draw (B) node[below]{$B$};
				\draw (F) node[right]{$F$};
				\draw (C) node[right]{$C$};
				\draw (G) node[above]{$G$};
				\draw (D) node[above]{$D$};
				\draw (H) node[left]{$H$};
				\draw (O) node[xshift=0cm, yshift=0cm]{$c^2$};
				\draw (A) -- (E)node[midway, below]{$a$};
				\draw (E) -- (B)node[midway, below]{$b$};
				\draw (B) -- (F)node[midway, right]{$a$};
				\draw (F) -- (C)node[midway, right]{$b$};
				\draw (C) -- (G)node[midway, above]{$a$};
				\draw (G) -- (D)node[midway, above]{$b$};
				\draw (D) -- (H)node[midway, left]{$a$};
				\draw (H) -- (A)node[midway, left]{$b$};
				\draw (E) -- (F)node[midway, below]{$c$};
				\draw (F) -- (G)node[midway, right]{$c$};
				\draw (G) -- (H)node[midway, above]{$c$};
				\draw (H) -- (E)node[midway, left]{$c$};
			\end{tikzpicture}
		\end{center}
	\end{proof}
	\begin{proposition}
		$\sin^2(x)+\cos^2(x)=1$
	\end{proposition}
\end{myleftlinebox}

\begin{myleftlinebox}
	some simple relations
	\tcblower
	\begin{itemize}
		\item for any triangle with sides of length $a$, $b$, and $c$: $a+b>c$, $b+c>a$, and $c+a>b$
		\item when $x$ is close to $0$, we have $\sin(x)<x<\tan(x)$
		\begin{center}
			\begin{tikzpicture}[
				my angle/.style = {
					draw, angle radius=7mm, 
					angle eccentricity=1.1, 
					right, inner sep=1pt,
					font=\footnotesize
					},scale=2
				]
				\coordinate (O) at (0,0);
				\coordinate (A) at (3,0);
				\coordinate (B) at (30:3);
				\coordinate (C) at (2.6,0);
				\coordinate (D) at (3,1.7);
				\draw (A) node[below]{$A$};
				\draw (O) node[below]{$O$};
				\draw (B) node[above]{$B$};
				\draw (D) node[above]{$D$};
				\draw (O) -- (A)node[midway,below]{$OA=r=1$};
				\draw (O) -- (B);
				\draw (A) arc (0:30:3)node[midway,left]{$x$};
				\draw (B) -- (intersection of 0,0 -- 3,0 and 30:3--330:3)node[midway,left]{$\sin(x)$};
				\draw (A) -- (intersection of 3,0 -- 3,3 and 0,0--30:3)node[midway,right]{$\tan(x)$};
				\draw pic[draw, angle radius=3mm] {right angle=O--C--B};
				\draw[dashed] (B) --(intersection of 3,0--3,5 and 0,0--30:3);
				\pic[my angle,"$x$"] {angle = A--O--B};
				\draw (C) node[below]{$C$};
				\draw (O) -- (C)node[xshift=-1.5cm, yshift=0.2cm,align=center]{$OC=\cos(x)$};
			\end{tikzpicture}
		\end{center}
		\item $\tan(x)=\frac{\sin(x)}{\cos(x)}$
		\item $\sin(x+2\pi)=\sin(x)$, $\cos(x+2\pi)=\cos(x)$
		\item $\sin(-x)=-\sin(x)$, $\cos(-x)=\cos(x)$, $\tan(-x)=-\tan(x)$
		\item $\sin(x+\pi)=-\sin(x)$, $\cos(x+\pi)=-\cos(x)$
		\item $\sin(x+\pi/2)=\cos(x)$, $\cos(x+\pi/2)=-\sin(x)$
	\end{itemize}
	
\end{myleftlinebox}

\begin{myleftlinebox}
	$\sin(x+y)$ and $\cos(x+y)$
	\tcblower
	\begin{center}
		\usetikzlibrary{calc}
		\begin{tikzpicture}[
			my angle/.style = {
				draw, angle radius=7mm, 
				angle eccentricity=1.1, 
				right, inner sep=1pt,
				font=\footnotesize
				}
			]
			\coordinate (A) at (0,0);
			\coordinate (B) at (3,0);
			\coordinate (C) at (3,2);
			\coordinate (D) at (3,5);
			\draw (A) node[below]{$A$};
			\draw (B) node[below]{$B$};
			\draw (C) node[right]{$C$};
			\draw (D) node[above]{$D$};
			\draw (A) -- (B);
			\draw (A) -- (C);
			\draw (A) -- (D)node[midway,left]{$AD=1$};
			\draw (D) -- (B);
			\pic[my angle,"$x$"] {angle = B--A--C};
			\pic[my angle,"$y$"] {angle = C--A--D};
			\draw pic[draw, angle radius=3mm] {right angle=A--B--D};
			
			\coordinate (E) at ($(A)!(D)!(C)$);
			\draw (E) node[right]{$E$};
			\draw (E) -- (C);
			\draw (E) -- (D);
			\draw pic[draw, angle radius=3mm] {right angle=A--E--D};

			\coordinate (F) at ($(A)!(E)!(B)$);
			\draw (F) node[right]{$F$};
			\draw (E) -- (F);
			\draw (F) -- (B);
			\draw pic[draw, angle radius=3mm] {right angle=E--F--B};

			\coordinate (G) at ($(C)!(E)!(D)$);
			\draw (G) node[left]{$G$};
			\draw (E) -- (G);
			\draw pic[draw, angle radius=3mm] {right angle=E--G--D};
		\end{tikzpicture}
	\end{center}
	From above figure, we can write the following:
	\begin{equation*}
		\begin{split}
			&DB=\sin(x+y)=DG+GB=DG+EF\\
			&AB=\cos(x+y)=AF-AB=AF-EG\\
			&\angle CDE = \angle CAB=x\\
			&DE=AD\sin(y)=\sin(y),DG=DE\cos(x)=\sin(y)\cos(x),EG=DE\sin(x)=\sin(y)\sin(x)\\
			&AE=AD\cos(y)=\cos(y),EF=AE\sin(x)=\cos(y)\sin(x), AF=AE\cos(x)=\cos(y)\cos(x)\\
			&\sin(x+y)=\sin(x)\cos(y)+\cos(x)\sin(y)\\
			&\cos(x+y)=\cos(x)\cos(y)-\sin(x)\sin(y)
		\end{split}
	\end{equation*}
\end{myleftlinebox}

\begin{myleftlinebox}
	other formulas 
	\tcblower
	\begin{equation*}
		\begin{split}
			\tan(x+y) &= \frac{\sin(x+y)}{\cos(x+y)}=\frac{\sin(x)\cos(y)+\cos(x)\sin(y)}{\cos(x)\cos(y)-\sin(x)\sin(y)}\\
			&= \frac{\tan(x)+\tan(y)}{1-\tan(x)\tan(y)}\\
			\sin(x-y)&= \sin(x+(-y)) = \sin(x)\cos(y)-\cos(x)\sin(y)\\
			\cos(x-y)&= \cos(x+(-y)) = \cos(x)\cos(y)+\sin(x)\sin(y)\\
			\tan(x-y)&= \tan(x+(-y)) =  \frac{\tan(x)-\tan(y)}{1+\tan(x)\tan(y)}\\
			\sin(2x) &= \sin(x+x) = 2\sin(x)\cos(x)=\frac{2\sin(x)\cos(x)}{\sin^2(x)+\cos^2(x)} = \frac{2\tan(x)}{1+\tan^2(x)}\\
			\cos(2x) &= \cos(x+x) = \cos^2(x)-\sin^2(x)=\frac{\cos^2(x)-\sin^2(x)}{\sin^2(x)+\cos^2(x)} = \frac{1-\tan^2(x)}{1+\tan^2(x)}\\
			\tan(2x) &= \tan(x+x) = \frac{2\tan(x)}{1-\tan^2(x)}
		\end{split}
	\end{equation*}
\end{myleftlinebox}

\begin{myleftlinebox}
	half-angle formulas 
	\tcblower
	use the identity:
	\begin{equation*}
		\begin{split}
			\cos(2x)&=2\cos^2(x)-1=1-2\sin^2(x)\\
			\cos(x) &=2\cos^2(x/2)-1=1-2\sin^2(x/2)
		\end{split}
	\end{equation*}
	then solve this quadratic equation we have
	\begin{equation*}
		\begin{split}
			\sin(x/2) &= \sqrt{\frac{\cos(x)+1}{2}} \text{ or } -\sqrt{\frac{\cos(x)+1}{2}}\\
			\cos(x/2) &= \sqrt{\frac{1-\cos(x)}{2}} \text{ or } -\sqrt{\frac{1-\cos(x)}{2}}
		\end{split}
	\end{equation*}
	where the sign can be determined using the quadrant of the half-angle.  
\end{myleftlinebox}

\begin{myleftlinebox}
	Law of sines
	\tcblower
	\begin{theorem}
		For any triangle $\triangle ABC$ with sides of length $a$, $b$, $c$, we have the following:
		\[\frac{a}{\sin(\angle A)}=\frac{c}{\sin(\angle C)}=\frac{b}{\sin(\angle B)}\]
		\begin{center}
			\begin{tikzpicture}
				\coordinate (A) at (0,0);
				\coordinate (B) at (3,0);
				\coordinate (C) at (2,2);
				\draw (A) node[below]{$A$};
				\draw (B) node[below]{$B$};
				\draw (C) node[above]{$C$};
				\draw (A) -- (B)node[midway,below]{$c$};
				\draw (A) -- (C)node[midway,left]{$b$};
				\draw (C) -- (B)node[midway,right]{$a$};
			\end{tikzpicture}
		\end{center}
	\end{theorem}
	The proof uses the fact that the area of this triangle $S=\frac{1}{2}c\cdot b\sin\angle A=\frac{1}{2}c\cdot a\sin\angle B$
\end{myleftlinebox}

\begin{myleftlinebox}
	Law of cosines
	\tcblower
	\begin{theorem}
		For any triangle $\triangle ABC$ with sides of length $a$, $b$, $c$, we have the following:
		\begin{align*}
			c^2 &= a^2+b^2 -2ab\cos\angle C\\
			a^2 &= b^2+c^2 -2bc\cos\angle A\\
			b^2 &= c^2+a^2 -2ca\cos\angle B
		\end{align*}
	\end{theorem}
	\begin{proof}
		Notice that $c=a\cos\angle B+b\cos\angle A$, we multiply this by $c$ and obtain
		\[c^2=ac\cos\angle B+bc\cos\angle A\]
		Do this for all three sides and we have
		\begin{align*}
			a^2 &= ac\cos\angle B+ab\cos\angle C\\
			b^2 &= bc\cos\angle A+ba\cos\angle C\\
			c^2 &= ca\cos\angle B+cb\cos\angle A
		\end{align*}
		And the rest part of the proof is obvious.
	\end{proof}
\end{myleftlinebox}

\section{Extensions}

\begin{myleftlinebox}
	inverse trigonometric functions, not the reciprocal trigonometric functions
	\tcblower
	With $y=\sin(x)$, where $x\in \bR$, we define $x=\arcsin(y)$ where $y\in[-1,1]$ and range $x\in [-\frac{\pi}{2},\frac{\pi}{2}]$. Similarly we can define the following:
	\begin{itemize}
		\item $y=\arcsin(x)$ where $x\in[-1,1]$ and $y\in [-\frac{\pi}{2},\frac{\pi}{2}]$
		\item $y=\arccos(x)$ where $x\in[-1,1]$ and $y\in [0,\pi]$
		\item $y=\arctan(x)$ where $x\in\bR$ and $y\in [-\frac{\pi}{2},\frac{\pi}{2}]$
	\end{itemize}
\end{myleftlinebox}

\begin{myleftlinebox}
	composition of inverse trigonometric functions
	\tcblower
	We have the following result:
	\begin{center}
		\begin{tabular}{lll}
			$\sin(\arcsin(x))=x$ & $\cos(\arcsin(x))=\sqrt{1-x^2}$ & $\sin(\arccos(x))=\sqrt{1-x^2}$\\
			$\sin(\arccos(x))=\sqrt{1-x^2}$ & $\cos(\arccos(x))=x$ & $\tan(\arccos(x))=\frac{\sqrt{1-x^2}}{x}$\\
			$\sin(\arctan(x))=\frac{x}{\sqrt{1+x^2}}$ & $\cos(\arctan(x))=\frac{1}{\sqrt{1+x^2}}$ & $\tan(\arctan(x))=x$
		\end{tabular}
	\end{center}
\end{myleftlinebox}

\begin{myleftlinebox}
	relation between inverse trigonometric functions
	\tcblower
	We have the following result:
	\begin{align*}
		\arcsin(-x) &= -\arcsin(x)\\
		\arccos(-x) &= \pi-\arccos(x)\\
		\arctan(-x) &= -\arctan(x)\\
		\arccos(x) &= \frac{\pi}{2}-\arcsin(x)\\
		\arctan(\frac{1}{x}) &= \frac{\pi}{2}- \arctan(x), x>0\\
		\arctan(\frac{1}{x}) &= -\frac{\pi}{2}- \arctan(x), x<0
	\end{align*}
\end{myleftlinebox}

\begin{myleftlinebox}
	hyperbolic functions
	\tcblower
	Using exponential function $e^x$ we define:
	\begin{align*}
		\sinh(x) &= \frac{e^x-e^{-x}}{2} = \frac{e^{2x}-1}{2e^x} = \frac{1-e^{-2x}}{2e^{-x}}\\
		\cosh(x) &= \frac{e^x+e^{-x}}{2} = \frac{e^{2x}+1}{2e^x} = \frac{1+e^{-2x}}{2e^{-x}}\\ 
		\tanh(x) &= \frac{\sinh(x)}{\cosh(x)} = \frac{e^x-e^{-x}}{e^x+e^{-x}} = \frac{e^{2x}-1}{e^{2x}+1}
	\end{align*}
\end{myleftlinebox}

\begin{myleftlinebox}
	relation between hyperbolic functions
	\tcblower
	Using exponential function $e^x$ we define:
	\begin{align*}
		\sinh(-x) &= -\sinh(x)\\
		\cosh(-x) &= \cosh(x)\\
		\cosh^2(x) -\sinh^2(x) &= 1\\
		\cosh(x)+\sinh(x)&=e^x\\
		\cosh(x)-\sinh(x)&=e^{-x}\\
		\sinh(x+y) &=\sinh(x)\cosh(y)+\cosh(x)\sinh(y)\\
		\cosh(x+y) &=\cosh(x)\cosh(y)+\sinh(x)\sinh(y)\\
		\arcsinh(x)&=\ln(\sqrt{x+\sqrt{x^2+1}})\\
		\arccosh(x)&=\ln(\sqrt{x+\sqrt{x^2-1}})\\
	\end{align*}
\end{myleftlinebox}

\section{Exercises}

\begin{myleftlinebox}
	show that $\frac{\sin(x)}{x}\to 1$ as $x\to 0$.
	\tcblower
	\vspace{2em}
\end{myleftlinebox}

\begin{myleftlinebox}
	show that $\frac{1-\cos(x)}{0.5x^2}\to 1$ as $x\to 0$.
	\tcblower
	\vspace{2em}
\end{myleftlinebox}

\begin{myleftlinebox}
	show that $\frac{\tan(x)}{x}\to 1$ as $x\to 0$.
	\tcblower
	\vspace{2em}
\end{myleftlinebox}

\end{document}
