\documentclass{article}

\input{D:/Notes/others/myHeadings.tex}

\title{HW0}
\author{Yuanxing Cheng, A20453410, CS577-f22}

\begin{document}

\maketitle

\section*{A}

let \(a = \SB{1,2,3}^\top\), \(b = \SB{4,5,6}^\top\), \(c = \SB{-1,1,3}^\top\).
\subsection*{1}

\begin{myleftlinebox}
    Find \(2a-b\)
    \tcblower
    \[
        2a-b = \SB{2\cdot 1-4,2\cdot 2-5,2\cdot 3-3 }^\top = \SB{-2,-1,0}^\top
    \]
\end{myleftlinebox}


\subsection*{2}
\begin{myleftlinebox}
    Find \(\hat a\) the unit vector along \(a\)
    \tcblower
    \[
        \hat a = \frac{a}{\abs{a}} = \frac{\SB{1,2,3}^\top}{\sqrt{1^2+2^2+3^2}}=\SB{\frac{1}{\sqrt{14}},\frac{2}{\sqrt{14}},\frac{3}{\sqrt{14}}}
    \]
\end{myleftlinebox}


\subsection*{3}
\begin{myleftlinebox}
    Find \(\norm a\) and teh angle of \(a\) relative to positive \(x\) axis
    \tcblower
    \[
        \norm{a} = \norm{a}_2 = \sqrt{1^2+2^2+3^2} = \sqrt{14}
    \]
    \[
        \theta = \arccos\Pare{\frac{a\cdot i}{\abs{a}\abs{i}}} = \arccos\Pare{\frac{1\cdot 1+2\cdot 0+3\cdot 0}{\sqrt{14}\cdot 1}} = \arccos\frac{1}{\sqrt{14}}
    \]
\end{myleftlinebox}



\subsection*{4}
\begin{myleftlinebox}
    Find direction cosines of \(a\)
    \tcblower
    \begin{align*}
        \theta_1 &= \theta = \arccos\Pare{1/\sqrt{14}}\\
        \theta_2 &= \arccos\Pare{\frac{a\cdot j}{\abs{a}\abs{i}}} = \arccos\Pare{\frac{1\cdot 0+2\cdot 1+3\cdot 0}{\sqrt{14}\cdot 1}} = \arccos\Pare{\frac{2}{\sqrt{14}}}\\
        \theta_3 &= \arccos\Pare{\frac{a\cdot k}{\abs{a}\abs{i}}} = \arccos\Pare{\frac{1\cdot 0+2\cdot 0+3\cdot 1}{\sqrt{14}\cdot 1}} = \arccos\Pare{\frac{3}{\sqrt{14}}}
    \end{align*}
\end{myleftlinebox}


\subsection*{5}
\begin{myleftlinebox}
    Find angle between \(a\) and \(b\)
    \tcblower
    \[
        \theta_{a,b} = \arccos\Pare{\frac{a\cdot b}{\abs{a}\cdot\abs{b}}}=\arccos\Pare{\frac{1\cdot 4+2\cdot 5+3\cdot 6}{\sqrt{14}\cdot \sqrt{4^2+5^2+6^2}}} = \Pare{\frac{32}{7\sqrt{22}}}
    \]
\end{myleftlinebox}


\subsection*{6}
\begin{myleftlinebox}
    Find \(a\cdot b\) and \(b\cdot a\)
    \tcblower
    \[
        a\cdot b = b\cdot a = 1\cdot 4+2\cdot 5+3\cdot 6 = 32
    \]
\end{myleftlinebox}


\subsection*{7}
\begin{myleftlinebox}
    Find \(a\cdot b\) by using the angle between \(a\) and \(b\)
    \tcblower
    \[
        a \cdot b = \abs{a}\abs{b}\cos \theta_{a,b} = 7\sqrt{22} \cdot \frac{32}{7\sqrt{22}} = 32
    \]
\end{myleftlinebox}


\subsection*{8}
\begin{myleftlinebox}
    The scalar projection of \(b\) onto \(\hat a\)
    \tcblower
    \[
        \abs{\Proj\Pare{b;\hat a}} = b\cdot \hat a = \frac{32}{\sqrt{14}}
    \]
    checking,
    \[
        \Proj\Pare{b;\hat a} = \frac{a a^\top}{a^\top a}b = \begin{bmatrix}
            1 & 2 & 3\\
            2 & 4 & 6\\
            3 & 6 & 9
        \end{bmatrix}b/\abs{a}^2 = \SB{32,64,96}^\top/14 = \SB{16/7,32/7,48/7}^\top
    \]
\end{myleftlinebox}



\subsection*{9}
\begin{myleftlinebox}
    Find a vector which is perpendicular to both \(a\)
    \tcblower
    consider \(x=[0,-3,x_3]^\top\) and then since \(x\) is perpendicular to \(a\), we have

    \[
        0 = x\cdot a = -3\cdot 2 + 3x_3\implies x_3 = 2
    \]

    so \(x =[0,-3,2]^\top\perp a\)
\end{myleftlinebox}


\subsection*{10}
\begin{myleftlinebox}
    Find \(a\times b\) and \(b\times a\)
    \tcblower
    using matrix notation

    \[
        a\times b = \begin{bmatrix}
            i & j & k\\
            1 & 2 & 3\\
            4 & 5 & 6
        \end{bmatrix} = -3i-(-6)j + (-3)k =[-3,6,-3]^\top
    \]  

    \[
    b\times a = - a\times b = [3,-6,3]^\top
    \]  
\end{myleftlinebox}



\subsection*{11}
\begin{myleftlinebox}
    Find a vector which is perpendicular to both \(a \) and \(b\)
    \tcblower
    \(a\times b\) is perpendicular to both vectors
\end{myleftlinebox}



\subsection*{12}
\begin{myleftlinebox}
    Find the linear dependency between these vecs
    \tcblower
    notice \(b-3a+c = 0\), thus they are linearly dependent.

\end{myleftlinebox}


\subsection*{13}
\begin{myleftlinebox}
    Find \(a^\top b\) and \(ab^\top\)
    \tcblower
    \[
        a^\top b = a\cdot b = 32, ab^\top = \begin{bmatrix}
            4 & 5 & 6\\
            8 & 10 & 12\\
            12 & 15 & 18
        \end{bmatrix}
    \]

\end{myleftlinebox}



\section*{B}

\(
    A = \begin{bmatrix}
        1 & 2 & 3\\
        4 & -2 & 3\\
        0 & -5 & 1
    \end{bmatrix}
\), \(B=\begin{bmatrix}
    1 & 2 & 1\\
    2 & 1 & -4\\
    3 & -2 & 1
\end{bmatrix}\), \(C = \begin{bmatrix}
    1 & 2 & 3\\
    4 & 5 & 6\\
    -1 & 1 & 3
\end{bmatrix}\), \(d = [1,2,3]^\top\)

\subsection*{1}
\begin{myleftlinebox}
    Find \(2A-B\)
    \tcblower
    using elementwise operation
    \[
        2A-B = \begin{bmatrix}
            1 & 2 & 5\\
            6 & -5 & 10\\
            -3 & 12 & -3
        \end{bmatrix}
    \]
\end{myleftlinebox}


\subsection*{2}
\begin{myleftlinebox}
    Find \(AB\) and \(BA\)
    \tcblower
    \[
        AB = \begin{bmatrix}
            14 & -2 & -4\\
            9 & 0 & 15\\
            7 & 7 & -21
        \end{bmatrix}, BA =  \begin{bmatrix}
            9 & 3 & 8\\
            6 & -18 & 13\\
            -5 & 15 & 2
        \end{bmatrix}
    \]
\end{myleftlinebox}


\subsection*{3}
\begin{myleftlinebox}
    Find \(\Pare{AB}^\top\) and \(B^\top A^\top\)
    \tcblower
    \[
        \Pare{AB}^\top = \begin{bmatrix}
            14 & 9 & 7\\
            -2 & 0 & 7\\
            -4 & 15 & -21
        \end{bmatrix}, B^\top A^\top = \Pare{AB}^\top
    \]
\end{myleftlinebox}


\subsection*{4}
\begin{myleftlinebox}
    Find \(\abs{A}\) and \(\abs{C}\)
    \tcblower
    \[
        a\cdot b = b\cdot a = 1\cdot 4+2\cdot 5+3\cdot 6 = 32
    \]
\end{myleftlinebox}
Notice \(C\) is from last problem whose row vectors are linearly dependent, thus has \(0\) determinant.
\[
    \abs{A}=2+0+60-0-(-8)-15 = 55, \abs{C}=0
\]

\subsection*{5}
\begin{myleftlinebox}
    Find whose matrix row vecs form an orthogonal set
    \tcblower
    \[
        a\cdot b = b\cdot a = 1\cdot 4+2\cdot 5+3\cdot 6 = 32
    \]
\end{myleftlinebox}

for \(A\), \(a^{row}_2\cdot a^{row}_3 = -13\) thus \(A\) is not; \(C\) not full rank, thus not. Now check \(B\), 
\begin{align*}
    b^{row}_2\cdot b^{row}_3 & = 6-2-4=0\\
    b^{row}_1\cdot b^{row}_3 & =3-4+1=0\\
    b^{row}_2\cdot b^{row}_1 & =2+2-4=0
\end{align*}

\subsection*{6}
\begin{myleftlinebox}
    Find \(A^{-1}\) and \(B^{-1}\)
    \tcblower
    Using adjoint  matrices.

    \[
        A^{-1} =\frac{1}{55}\begin{bmatrix}
            2-15 & -(-2)+15 & 6-(-6)\\
            -(-4)+0 & -1-0 & -3+12\\
            20-0 & -5+0 & -2-8
        \end{bmatrix} = \begin{bmatrix}
            -13/55 & 17/55 & 12/55\\
            4/55 & -1/55 & 9/55\\
            4/11 & -1/11 & -2/11
        \end{bmatrix},
    \]

    \[
        B^{-1}	 = \frac{1}{-42}\begin{bmatrix}
            1-8 & -2+(-2) & -8-1\\
            -2+(-12) & 1-3 & -(-4)+2\\
            -4-3 & -(-2)+6 & 1-4
        \end{bmatrix} = \begin{bmatrix}
            1/6 & 2/21 & 3/14\\
            1/3 & 1/21 & -1/7\\
            1/6 & -4/21 & 1/14
        \end{bmatrix}
    \]
\end{myleftlinebox}

\subsection*{7}
\begin{myleftlinebox}
    Find \(C^{-1}\)
    \tcblower
    As row's are linearly dependent, inverse didn't exist. 

\end{myleftlinebox}

\subsection*{8}
\begin{myleftlinebox}
    Find \(Ad\)
    \tcblower
    \[
        Ad = [14,9,7]^\top
    \]
\end{myleftlinebox}


\subsection*{9}
\begin{myleftlinebox}
    Find the scalar projection of the rows of \(A\) onto the vector \(d\) with noralizing \(d\)
    \tcblower
    \[
        A\hat d= [\sqrt{14},9/\sqrt{14},7/\sqrt{14}]^\top
    \]
\end{myleftlinebox}


\subsection*{10}
\begin{myleftlinebox}
    Find the vector projection of the rows of \(A\) onto the vector \(d\) with noralizing \(d\)
    \tcblower
    \[
        \Proj\Pare{A;\hat d}^\top = \Pare{\frac{d d^\top}{d^\top d}A^\top}^\top =\frac{1}{d^\top d}A d d^\top= A \begin{bmatrix}
            1 & 2 & 3\\
            2 & 4 & 6\\
            3 & 6 & 9
        \end{bmatrix}/\abs{d}^2 =  \begin{bmatrix}
            \sqrt{14} & 2\sqrt{14} & 3\sqrt{14}\\
            9/\sqrt{14} & 18/\sqrt{14} & 27/\sqrt{14} \\
            7/\sqrt{14} & \sqrt{14} & 21/\sqrt{14}
        \end{bmatrix}
    \]
\end{myleftlinebox}



\subsection*{11}
\begin{myleftlinebox}
    Find linear combination of the columns of \(A\) using the elements of \(d\)
    \tcblower
    \[
        Ad = [14,9,7]^\top
    \]
\end{myleftlinebox}



\subsection*{12}
\begin{myleftlinebox}
    Find \(x\) for \(Bx=d\)
    \tcblower
    Notice \(B=[d,e,f]\) so if \(x = [x_1,x_2,x_3]^\top\),

    \[
        x_1 d+x_2 e+x_3 f = d \implies x=[1,0,0]^\top
    \]

    Since \(B\) nonsingular, so that's the only solution.

\end{myleftlinebox}


\subsection*{13}
\begin{myleftlinebox}
    Find \(x\) for \(Cx=d\) and reason
    \tcblower
    Using Gaussian elimination we end up with

    \[
        \begin{bmatrix}
            1 & 2 & 3\\
            0 & -3 & -6\\
            0 & 3 & 6
        \end{bmatrix} [x_1,x_2,x_3]^\top = [1, -2,4]^\top
    \]
    Seeing last rows we know there's no such \(x\) satisfies the equation.

\end{myleftlinebox}

\section*{C}
\(
    D = \begin{bmatrix}
        1 & 2\\
        3 & 2
    \end{bmatrix}
\), \(E =\begin{bmatrix}
    2 & -2 \\
    -2 & 5
\end{bmatrix}\), \(F = \begin{bmatrix}
    1 & 2\\
    2 & 4
\end{bmatrix}\)
\subsection*{1}
\begin{myleftlinebox}
    Find eigenvalues and eigenvectors of \(D\)
    \tcblower
    \[
        \det\Pare{\lambda I-D } = (\lambda-1)(\lambda -2)-6 = (\lambda-4)(\lambda+1)
    \]
    so the eigenvalues are \(-1\) and \(4\), then solve eigenvectors,
    \[
        \Pare{- I-D }x = 0 \implies x = [1,-1]^\top
    \]
    \[
        \Pare{4 I-D }x = 0 \implies x = [2,3]^\top
    \]
\end{myleftlinebox}


\subsection*{2}
\begin{myleftlinebox}
    Find the dot product between the eigenvalues of \(D\)
    \tcblower
    \[
        1\cdot 2-1\cdot 3 = -1
    \]
\end{myleftlinebox}

\subsection*{3}
\begin{myleftlinebox}
    Find the dot product between the eigenvalues of \(E\)
    \tcblower
    \[
        \det\Pare{\lambda I-E } = (\lambda-2)(\lambda -5)-4 = (\lambda-6)(\lambda-1)=0\implies \lambda_1 = 1,\lambda_2=6
    \]
    \[
        \Pare{I-E }x = 0 \implies x = [2,1]^\top
    \]
    \[
        \Pare{6I-E }x = 0 \implies x = [-1,2]^\top
    \]
    \[
        -2+2=0
    \]
\end{myleftlinebox}


\subsection*{4}
\begin{myleftlinebox}
    Find the property of the eigenvalues of \(E\) and reason
    \tcblower
    the eigenvectors of \(E\) are orthogonal due to the fact that \(E\) is symmetric. Reason

    Let \(Ex = \lambda_1 x\) and \(Ey = \lambda_2 y\) where \(\lambda_1\neq \lambda_2\) we have

    \begin{equation}\label{eqn:symM_eig_Ortho}
        \begin{split}
            \lambda_1 x\cdot y & = Ex \cdot y\\
            &= (Ex)^\top y = x^\top Ey \\
            & = x\cdot (Ey) = x\cdot \lambda_2 y\\
            \implies (\lambda_1 - \lambda_2)x\cdot y &= 0
        \end{split}
    \end{equation}
    Since we've assumed \(\lambda_1\neq \lambda_2\), \(x\cdot y=0\) thus orthogonal.

\end{myleftlinebox}

\subsection*{5}
\begin{myleftlinebox}
    Find trivial \(x\) for \(Fx=0\)
    \tcblower
    Trivial solution for \(Fx=0\) is just zero vector \([0,0]^\top\).
\end{myleftlinebox}


\subsection*{6}
\begin{myleftlinebox}
    Find non-trivial \(x\) for \(Fx=0\)
    \tcblower
    non trivial solution, we can have \(x=[2,-1]^\top\) or  \(x=[4,-2]^\top\)
\end{myleftlinebox}

\section*{7}
\begin{myleftlinebox}
    the only solution \(x\) to \(Dx=0\) and reason why single solution
    \tcblower
    it only has trivial solution \([0,0]^\top\). Reason is by gaussian elimination or null space dimention equals to \(n-rank(D)=2-2=0\) thus null space contains only zero vector.
\end{myleftlinebox}

\section*{D}
\(f(x) = x^2+3\), \(g(x)=x^2\), \(q(x,y) = x^2+y^2\)
\subsection*{1}

\begin{myleftlinebox}
    first and second derivative of \(f\) wrt \(x\)
    \tcblower
    \[
        f'(x) = 2x, f''(x) = 2  
    \]
\end{myleftlinebox}

\subsection*{2}
\begin{myleftlinebox}
    partial derivatives of \(q\)
    \tcblower
    \[
        \frac{\partial q}{\partial x} =2x, \frac{\partial q}{\partial y} =2y
    \]
\end{myleftlinebox}

\subsection*{3}
\begin{myleftlinebox}
    gradient of \(q\)
    \tcblower
    \[
        \nabla q = [\frac{\partial q}{\partial x},\frac{\partial q}{\partial y}]^\top=[2x,2y]^\top
    \]
\end{myleftlinebox}

\subsection*{4}
\begin{myleftlinebox}
    the derivative of \(f\circ g\) wrt \(x\), with and without using chain rule
    \tcblower
    \[
        f\circ g(x) = x^4+3\implies \Pare{f\circ g}'(x) = 4x^3\\
        \Pare{f\circ g}'(x) = \given{\frac{\partial f(y)}{\partial y}}_{y=g(x)} \frac{\partial g(x)}{\partial x} = 2(x^2)*2x=4x^3
    \]
\end{myleftlinebox}

\subsection*{E}\
Doing A, B, C with python, see following notebook pdf.





\newpage

%\bibliographystyle{acm}
%\bibliography{D:/Papers.bib}

\newpage
\appendix
\section{Appendix}

\end{document}