{
 "cells": [
  {
   "cell_type": "markdown",
   "metadata": {},
   "source": [
    "# <center>Models and Pricing of Financial Derivatives HW_03</center>\n",
    "\n",
    "**<center>11510691 程远星$\\DeclareMathOperator*{\\argmin}{argmin}\n",
    "\\DeclareMathOperator*{\\argmax}{argmax}\n",
    "\\DeclareMathOperator*{\\plim}{plim}\n",
    "\\newcommand{\\using}[1]{\\stackrel{\\mathrm{#1}}{=}}\n",
    "\\newcommand{\\ffrac}{\\displaystyle \\frac}\n",
    "\\newcommand{\\asim}{\\overset{\\text{a}}{\\sim}}\n",
    "\\newcommand{\\space}{\\text{ }}\n",
    "\\newcommand{\\bspace}{\\;\\;\\;\\;}\n",
    "\\newcommand{\\QQQ}{\\boxed{?\\:}}\n",
    "\\newcommand{\\void}{\\left.\\right.}\n",
    "\\newcommand{\\Tran}[1]{{#1}^{\\mathrm{T}}}\n",
    "\\newcommand{\\d}[1]{\\displaystyle{#1}}\n",
    "\\newcommand{\\CB}[1]{\\left\\{ #1 \\right\\}}\n",
    "\\newcommand{\\SB}[1]{\\left[ #1 \\right]}\n",
    "\\newcommand{\\P}[1]{\\left( #1 \\right)}\n",
    "\\newcommand{\\abs}[1]{\\left| #1 \\right|}\n",
    "\\newcommand{\\norm}[1]{\\left\\| #1 \\right\\|}\n",
    "\\newcommand{\\dd}{\\mathrm{d}}\n",
    "\\newcommand{\\Exp}{\\mathrm{E}}\n",
    "\\newcommand{\\RR}{\\mathbb{R}}\n",
    "\\newcommand{\\EE}{\\mathbb{E}}\n",
    "\\newcommand{\\II}{\\mathbb{I}}\n",
    "\\newcommand{\\NN}{\\mathbb{N}}\n",
    "\\newcommand{\\ZZ}{\\mathbb{Z}}\n",
    "\\newcommand{\\QQ}{\\mathbb{Q}}\n",
    "\\newcommand{\\PP}{\\mathbb{P}}\n",
    "\\newcommand{\\AcA}{\\mathcal{A}}\n",
    "\\newcommand{\\FcF}{\\mathcal{F}}\n",
    "\\newcommand{\\AsA}{\\mathscr{A}}\n",
    "\\newcommand{\\FsF}{\\mathscr{F}}\n",
    "\\newcommand{\\Var}[2][\\,\\!]{\\mathrm{Var}_{#1}\\left[#2\\right]}\n",
    "\\newcommand{\\Avar}[2][\\,\\!]{\\mathrm{Avar}_{#1}\\left[#2\\right]}\n",
    "\\newcommand{\\Cov}[2][\\,\\!]{\\mathrm{Cov}_{#1}\\left(#2\\right)}\n",
    "\\newcommand{\\Corr}[2][\\,\\!]{\\mathrm{Corr}_{#1}\\left(#2\\right)}\n",
    "\\newcommand{\\I}[1]{\\mathrm{I}\\left( #1 \\right)}\n",
    "\\newcommand{\\N}[1]{\\mathcal{N} \\left( #1 \\right)}\n",
    "\\newcommand{\\ow}{\\text{otherwise}}\n",
    "\\newcommand{\\FSD}{\\text{FSD}}\n",
    "\\void^\\dagger$</center>**"
   ]
  },
  {
   "cell_type": "markdown",
   "metadata": {},
   "source": [
    "## Question 1\n",
    "\n",
    "$\\P{1}$\n",
    "\n",
    "$\\bspace \\begin{align}\n",
    "\\dd y &= \\dd\\P{2S_t}\\\\\n",
    "&= \\P{0 + \\P{\\mu S_t}\\cdot 2 + \\ffrac{1}{2}\\P{\\sigma S_t}^2  \\cdot 0}\\dd t + \\sigma S_t \\cdot 2 \\dd z\\\\\n",
    "&= 2\\mu S_t \\dd t + 2\\sigma S_t \\dd z\\\\\n",
    "&= \\mu y \\dd t + \\sigma y\\dd z\n",
    "\\end{align}$\n",
    "\n",
    "$\\P{2}$\n",
    "\n",
    "$\\bspace \\begin{align}\n",
    "\\dd y &= \\dd\\P{S_t^2}\\\\\n",
    "&= \\P{0 + \\P{\\mu S_t}\\cdot S_t + \\ffrac{1}{2}\\P{\\sigma S_t}^2  \\cdot 2}\\dd t + \\P{\\sigma S_t} \\cdot S_t \\dd z\\\\\n",
    "&= \\P{2\\mu S_t^2 + \\sigma^2 S_t^2}\\dd t + 2\\sigma S_t^2 \\dd z\\\\\n",
    "&= \\P{2\\mu + \\sigma^2}y\\dd t + 2\\sigma y \\dd z\n",
    "\\end{align}$\n",
    "\n",
    "$\\P{3}$\n",
    "\n",
    "$\\bspace \\begin{align}\n",
    "\\dd y &= \\dd\\P{e^{S_t}}\\\\\n",
    "&= \\P{0 + \\P{\\mu S_t}\\cdot e^{S_t} + \\ffrac{1}{2}\\P{\\sigma S_t}^2  \\cdot e^{S_t}}\\dd t + \\P{\\sigma S_t} \\cdot e^{S_t} \\dd z\\\\\n",
    "&= \\P{\\mu \\log y + \\ffrac{1}{2} \\P{\\sigma \\log y}^2}y\\dd t + \\P{\\sigma \\log y} \\cdot y\\dd t\n",
    "\\end{align}$\n",
    "\n",
    "$\\P{4}$\n",
    "\n",
    "$\\bspace \\begin{align}\n",
    "\\dd y &= \\dd\\P{\\ffrac{e^{r\\P{T-t}}}{S_t}}\\\\\n",
    "&= \\P{\\ffrac{-re^{r\\P{T-t}}}{S_t} + \\P{\\mu S_t}\\cdot \\P{-\\ffrac{e^{r\\P{T-t}}}{S_t^2}} + \\ffrac{1}{2}\\P{\\sigma S_t}^2  \\cdot \\ffrac{2e^{r\\P{T-t}}}{S_t^3}}\\dd t + \\P{\\sigma S_t} \\cdot \\P{-\\ffrac{e^{r\\P{T-t}}}{S_t^2}} \\dd z\\\\\n",
    "&= \\P{-r-\\mu-\\sigma^2}y\\dd t - \\sigma y \\dd y\n",
    "\\end{align}$"
   ]
  },
  {
   "cell_type": "markdown",
   "metadata": {},
   "source": [
    "## Question 2\n",
    "\n",
    "$\\bspace$It is a Brownian motion, the four conditions are checked correct below. We first let the drift and volatility of $W_t$ and $\\widetilde W_t$ are $\\mu,\\sigma$ and $\\check\\mu,\\check\\sigma$, respectively. Denote $\\widehat W_t$ as the standard Brownian motion, then $\\forall\\; t>s$, we have\n",
    "\n",
    "$$\\begin{align}\n",
    "X_t - X_s  &= \\rho\\P{W_t - W_s} + \\sqrt{1-\\rho^2}\\P{\\widetilde W_t - \\widetilde W_s} \\\\\n",
    "&= \\rho\\P{\\mu \\P{t-s} + \\sigma \\P{\\widehat W_t-\\widehat W_s}} + \\sqrt{1-\\rho^2}\\P{\\check\\mu \\P{t-s} + \\check\\sigma \\P{\\widehat W_t - \\widehat W_s}}\\\\\n",
    "&= \\P{\\rho \\mu + \\sqrt{1-\\rho^2}\\check \\mu}\\P{t-s} + \\P{\\rho\\sigma + \\sqrt{1-\\rho^2}\\check\\sigma}\\P{\\widehat W_t - \\widehat W_s}\n",
    "\\end{align}$$\n",
    "\n",
    "- Let $\\rho \\mu + \\sqrt{1-\\rho^2}\\check \\mu \\equiv \\dot \\mu$ and $\\rho\\sigma + \\sqrt{1-\\rho^2}\\check\\sigma\\equiv\\dot\\sigma$, then \n",
    "\n",
    "$$X_t - X_s = \\dot\\rho\\P{t-s} + \\dot\\sigma\\P{W_t-W_s} \\sim \\N{\\dot\\rho\\P{t-s},\\dot\\sigma^2 \\P{t-s}},\\bspace\\forall\\; t>s$$\n",
    "\n",
    "- Consider $t$ and $s$ as two adjacent time in the interval $\\SB{0,T}$. Then since $\\widehat W_t$ has independent increments, so is $X_t - X_s$, judging from its expression.\n",
    "- $X_0 = \\dot\\rho t + \\dot\\sigma \\widehat W_t \\mid_{t=0} = \\widehat W_0 = 0$\n",
    "- Still, from the expression of $X_t$, $t$ is continuous and the path $\\SB{W_t:t\\geq 0}$ are also continuous functions, $X_t$ is continuous."
   ]
  },
  {
   "cell_type": "markdown",
   "metadata": {},
   "source": [
    "## Question 3\n",
    "\n",
    "$\\P{1}$\n",
    "\n",
    "$\\bspace$It is a $\\PP$-Brownian motion.\n",
    "\n",
    "- $\\forall\\; t>s$, the increment $\\P{-W_t} - \\P{-W_s} = W_s - W_t$ also has the normal distribution $\\N{0,t-s}$\n",
    "- The process $-W_t$ has independent increments: for any set of times $0\\leq t_1<t_2<\\cdots<t_n$, the $r.v.$ $-W_{t_{\\void_2}} + W_{t_{\\void_1}}$, $-W_{t_{\\void_3}} + W_{t_{\\void_2}}$, $\\dots$, $-W_{t_{\\void_{n}}} + W_{t_{\\void_{n-1}}}$ are also independent, since their inverse are.\n",
    "- $-W_0 = 0$\n",
    "- The sample paths: $\\SB{-W_t: t \\geq 0}$ are continuous function of $t$ since $\\SB{W_t: t \\geq 0}$ are.\n",
    "\n",
    "$\\P{2}$\n",
    "\n",
    "$\\bspace$It is a $\\PP$-Brownian motion.\n",
    "\n",
    "- $\\forall\\; t>s$, the increment $c\\P{W_{t/c^{\\void_2}}} - c\\P{W_{s/c^{\\void_2}}}$ also has the normal distribution $\\N{0,c^2\\P{t/c^2 - s/c^2}} = \\N{0,t-s}$\n",
    "- The process $cW_{t/c^{\\void_2}}$ has independent increments: for any set of times $0\\leq t_1<t_2<\\cdots<t_n$, the $r.v.$ $-W_{t_{\\void_2}} + W_{t_{\\void_1}}$, $-W_{t_{\\void_3}} + W_{t_{\\void_2}}$, $\\dots$, $-W_{t_{\\void_{n}}} + W_{t_{\\void_{n-1}}}$ are also independent, since they are a subset of  $r.v.$ with time range from $0$ to $c^2 t_n$\n",
    "- $-cW_{0/c^{\\void_2}} = cW_0 = 0$\n",
    "- The sample paths: $\\SB{-W_{t/c^{\\void_2}}: t \\geq 0}$ are continuous function of $t$ since $\\SB{W_t: t \\geq 0}$ are, so that we can multiply a constant and rescale the time axis to its $1/c^2$ while keeping the continuity\n",
    "\n",
    "$\\P{3}$\n",
    "\n",
    "$\\bspace$It's not. We next prove this process doesn't have the independent increments. Here's the covariance if taking the time $0$, $s$, and $t$.\n",
    "\n",
    "$$\\begin{align}\n",
    "&\\Cov{\\sqrt{t} W_1 - \\sqrt s W_1, \\sqrt s W_1}\\\\\n",
    "=&\\; \\P{\\sqrt t - \\sqrt s}\\sqrt s \\cdot \\Var{W_1}\\\\\n",
    "=&\\; \\P{\\sqrt t - \\sqrt s}\\sqrt s \\neq 0\n",
    "\\end{align}$$\n",
    "\n",
    "$\\P{4}$\n",
    "\n",
    "$\\bspace$It's not. Still, let's see the covariance, taking the time $0$, $2s$ and $2t$.\n",
    "\n",
    "$$\\begin{align}\n",
    "   &\\Cov{\\P{W_{2t} - W_t}-\\P{W_{2s} - W_s}, W_{2s} - W_s}\\\\\n",
    "=\\;&\\Cov{\\P{W_{2t} - W_{2s}}-\\P{W_t - W_s}, W_{2s} - W_s}\\\\\n",
    "=\\;&\\Cov{W_{2t} - W_{2s},W_{2s}} + \\Cov{\\P{W_t - W_s}, W_s}\\\\\n",
    "\\;&\\bspace - \\Cov{W_{2t} - W_{2s},W_{s}} - \\Cov{\\P{W_t - W_s},W_{2s}}\\\\\n",
    "=\\;& 0+2\\Cov{W_{2s},W_s} - \\Cov{W_{2t},W_s} - \\Cov{W_{t},W_{2s}}\\\\\n",
    "=\\;& 0+2\\Cov{W_{2s} - W_s,W_s}+2\\Cov{W_s,W_s} - \\Cov{W_{2t}-W_s,W_s} + \\Cov{W_s,W_s} - \\Cov{W_{t},W_{2s}}\\\\\n",
    "=\\;& \\Var{W_s} - \\Cov{W_{t},W_{2s}} = s - \\Cov{W_{t},W_{2s}}\n",
    "\\end{align}$$\n",
    "\n",
    "$\\bspace$If $t > 2s$, then the preceding equals to $s - \\Var{W_{2s}} = -s \\neq 0$."
   ]
  },
  {
   "cell_type": "markdown",
   "metadata": {},
   "source": [
    "## Question 4\n",
    "\n",
    "$$\\begin{align}\n",
    "\\Exp\\SB{e^{\\theta X}} &= \\int^{\\infty}_{-\\infty} e^{\\theta X}\\cdot\\ffrac{1}{\\sqrt{2\\pi}\\sigma}\\exp\\CB{-\\ffrac{ \\P{x-\\mu}^2}{2\\sigma^2}}\\;\\dd x\\\\\n",
    "&= \\int^{\\infty}_{-\\infty} e^{\\theta X}\\cdot\\ffrac{1}{\\sqrt{2\\pi}\\sigma}\\exp\\CB{-\\ffrac{ \\P{x-\\mu+\\theta\\sigma^2}^2}{2\\sigma^2}} \\cdot\\exp\\CB{\\ffrac{\\theta^2\\sigma^2}{2} + \\theta\\mu}\\;\\dd x\\\\\n",
    "&= \\exp\\CB{\\ffrac{\\theta^2\\sigma^2}{2} + \\theta\\mu}\n",
    "\\end{align}$$\n",
    "\n",
    "$\\bspace$And to find $\\Exp\\SB{X^4} = \\left.\\ffrac{\\dd^4}{\\dd \\theta^4}\\Exp\\SB{e^{\\theta X}}\\right|_{\\theta=0}$, we let $f\\P{\\theta} = \\ffrac{\\theta^2\\sigma^2}{2} + \\theta\\mu$, then\n",
    "\n",
    "$$\\begin{align}\n",
    "\\ffrac{\\dd^4}{\\dd \\theta^4}\\Exp\\SB{e^{\\theta X}} &= \\ffrac{\\dd^3}{\\dd \\theta^3}\\P{f' e^f}\\\\\n",
    "&= \\ffrac{\\dd^2}{\\dd \\theta^2}\\P{\\P{f'^2 + f''} e^f}\\\\\n",
    "&= \\ffrac{\\dd}{\\dd \\theta}\\P{\\P{2f''f' + f^{\\P{3}}+f'} e^f}\\\\\n",
    "&= \\P{\\P{2f^{\\P{3}}f' + f^{\\P{4}}+f'+f''+2\\P{f''}^2} e^f}\n",
    "\\end{align}$$\n",
    "\n",
    "$\\bspace$Plug in $\\theta=0$ and by $f = 0 = f^{\\P{3}} = f^{\\P{4}}$, $f' = \\mu$, $f'' = \\sigma^2$, we have\n",
    "\n",
    "$$\\Exp\\SB{X^4} = 2\\sigma^4 + \\sigma^2 + \\mu$$"
   ]
  },
  {
   "cell_type": "markdown",
   "metadata": {},
   "source": [
    "## Question 5\n",
    "\n",
    "$\\P{1}$\n",
    "\n",
    "$\\bspace$It's not. Since $\\Exp\\SB{\\abs{e^{\\sigma W_t}}} = \\exp\\CB{\\ffrac{1}{2}\\sigma^2t} < \\infty$. Now see the second condition. \n",
    "\n",
    "$$\\begin{align}\n",
    "\\Exp_s\\SB{e^{\\sigma W_t}} &= \\Exp_s\\SB{e^{\\sigma W_s}\\cdot e^{\\sigma \\P{W_t-W_s}}}\\\\\n",
    "&= e^{\\sigma W_s} \\Exp_s\\SB{e^{\\sigma \\P{W_t-W_s}}} \\\\\n",
    "&= e^{\\sigma W_s} \\Exp\\SB{e^{\\sigma W_{t-s}}}\\\\\n",
    "&= \\exp\\CB{\\sigma W_s +\\ffrac{\\sigma^2}{2}\\P{t-s}} \\neq e^{\\sigma W_s}\n",
    "\\end{align}$$\n",
    "\n",
    "$\\P{2}$\n",
    "\n",
    "$\\bspace$It is, if only $c\\geq 1$ because if not then the process is not even adapted to the filtration. Now suppose $c\\geq1$, then $\\Exp\\SB{\\abs{cW_{t/c^{\\void_2}}}} \\leq \\Exp\\SB{\\ffrac{1+c^2W_{t/c^{\\void_2}}^2}{2}} = \\ffrac{1+ c^2\\cdot t/c^2}{2} = \\ffrac{1+t}{2} < \\infty$. Now see the second condition. \n",
    "\n",
    "$$\\begin{align}\n",
    "\\Exp_s\\SB{cW_{t/c^{\\void_2}}} &= cW_{s/c^{\\void_2}} + c\\Exp_s\\SB{W_{t/c^{\\void_2}} - W_{s/c^{\\void_2}}}\\\\\n",
    "&= cW_{s/c^{\\void_2}} + \\Exp\\SB{W_{\\P{t-s}/c^{\\void_2}}}\\\\\n",
    "&= cW_{s/c^{\\void_2}} \\\\\n",
    "&\\surd\n",
    "\\end{align}$$\n",
    "\n",
    "$\\P{3}$\n",
    "\n",
    "$\\bspace$It is. For the first condition,\n",
    "\n",
    "$$\\begin{align}\n",
    "\\Exp\\SB{\\abs{tW_t - \\d{\\int_{0}^{t} W_s\\;\\dd s}}} &\\leq  \\Exp\\SB{\\abs{tW_t} + \\abs{\\d{\\int_{0}^{t} W_s\\;\\dd s}}}\\\\\n",
    "&\\leq t\\cdot\\Exp\\SB{\\ffrac{W_t^2 + 1}{2}} + \\int_{0}^{t} \\Exp\\SB{\\abs{W_s}}\\;\\dd s\\\\\n",
    "&\\leq t\\cdot\\ffrac{1+t}{2} + \\int_{0}^{t} \\ffrac{1+s}{2}\\;\\dd s\\\\\n",
    "&= t + \\ffrac{3}{4}t^2 <\\infty\n",
    "\\end{align}$$ \n",
    "\n",
    "$\\bspace$And then the second one, in the review we have\n",
    "\n",
    "$$tW_t - \\int_{0}^{t} W_s\\;\\dd s = \\int_0^t s\\dd W_t$$\n",
    "\n",
    "$\\bspace$It's an Itô's process! Thus it's a martingale."
   ]
  },
  {
   "cell_type": "markdown",
   "metadata": {},
   "source": [
    "## Question 6\n",
    "\n",
    "$\\bspace$Following the three conditions that define the martingale, we have\n",
    "\n",
    "$$\\Exp\\SB{\\abs{f}}<\\infty\\\\\n",
    "\\Exp_s\\SB{f\\P{t,W_t}} = f\\P{s,W_s}$$\n",
    "\n",
    "$\\bspace$And to check this, it fails the second one\n",
    "\n",
    "$$\\Exp\\SB{\\abs{e^{vt + \\sigma W_t}}}= \\Exp\\SB{{e^{vt + \\sigma W_t}}} = \\exp\\CB{vt + \\ffrac{1}{2}\\sigma^2 t} < \\infty$$\n",
    "\n",
    "$$\\begin{align}\n",
    "\\Exp_s\\SB{e^{vt+\\sigma W_t}} &= e^{vs+\\sigma W_t}\\exp\\CB{\\ffrac{\\sigma^2}{2}t}\\Exp\\SB{e^{\\sigma\\P{W_t - W_s}}}\\\\\n",
    "&= \\exp\\CB{vt + \\ffrac{\\sigma^2}{2}\\P{t-s}+\\sigma W_s}\\neq e^{vs + \\sigma W_s}\n",
    "\\end{align}$$"
   ]
  },
  {
   "cell_type": "markdown",
   "metadata": {},
   "source": [
    "## Question 7\n",
    "\n",
    "$\\bspace$Firstly, it's adapted to $\\FcF_t$ and likewise we have $\\Exp\\SB{\\abs{I_n}} \\leq \\Exp\\SB{\\ffrac{I_n^2+1} {2}}<\\infty$. Then,\n",
    "\n",
    "$$\\begin{align}\n",
    "\\Exp_s\\SB{I\\P{t}} =& I\\P{s} + \\Exp_s\\SB{I\\P{t} - I\\P{s}} \\\\[0.6em]\n",
    "&\\bspace \\text{partition the interval } \\SB{s,t} \\text{ in } n \\text{ subintervals}\\\\[0.5em]\n",
    "=& I\\P{s} + \\Exp_s\\SB{ \\lim_{n\\to\\infty} \\sum_{j=0}^{n-1} h\\P{t_j, W_{t_{\\void_{j}}}}\\P{W_{t_{\\void_{j+1}}} - W_{t_{\\void_{j}}}} }\\\\[0.6em]\n",
    "&\\bspace \\text{assume the summation is exchangable with the expectation } \\\\[0.5em]\n",
    "=& I\\P{s} + \\lim_{n\\to\\infty} \\sum_{j=0}^{n-1} \\Exp_s\\SB{ h\\P{t_j, W_{t_{\\void_{j}}}}\\P{W_{t_{\\void_{j+1}}} - W_{t_{\\void_{j}}}} }\\\\[0.6em]\n",
    "&\\bspace \\text{condition on }\\FcF_{t_{\\void_{j}}}, \\Exp\\SB{X\\mid Y} = \\Exp\\SB{\\Exp\\SB{X \\mid Y,W} \\mid Y} \\\\[0.5em]\n",
    "=& I\\P{s} + \\lim_{n\\to\\infty} \\sum_{j=0}^{n-1} \\Exp_s\\SB{ \\Exp_{t_{\\void_{j}}}\\SB{ h\\P{t_j, W_{t_{\\void_{j}}}} \\P{W_{t_{\\void_{j+1}}} - W_{t_{\\void_{j}}}} } }\\\\\n",
    "=& I\\P{s} + \\lim_{n\\to\\infty} \\sum_{j=0}^{n-1} \\Exp_s\\SB{  h\\P{t_j, W_{t_{\\void_{j}}}} } \\Exp_{t_{\\void_{j}}} \\SB{{W_{t_{\\void_{j+1}}} - W_{t_{\\void_{j}}}} }\\\\[0.5em]\n",
    "=& I\\P{s}\n",
    "\\end{align}$$"
   ]
  },
  {
   "cell_type": "markdown",
   "metadata": {},
   "source": [
    "## Question 8\n",
    "\n",
    "$\\P{1}$\n",
    "\n",
    "$\\bspace$Let $X_t = W_t$, then\n",
    "\n",
    "$$\\begin{align}\\dd Y_t &= \\P{0 + 0 \\cdot 3X_t^2 + \\ffrac{1}{2}\\cdot1\\cdot6X_t}\\dd t + 1\\cdot 3 X_t^2 \\dd W_t\\\\\n",
    "&= 3X_t \\dd t + 3X_t^2 \\dd W_t\\\\\n",
    "&= 3\\sqrt[3]{Y_t} \\dd t + 3\\sqrt[3]{Y_t^2} \\dd W_t\n",
    "\\end{align}$$\n",
    "\n",
    "$\\bspace$It's not a martingale since\n",
    "\n",
    "$$\\begin{align}\n",
    "\\Exp_s\\SB{W_t^3} &= \\Exp_s\\SB{\\P{W_t - W_s + W_s}^3}\\\\\n",
    "&= \\Exp_s\\SB{\\P{W_t - W_s}^3} + \\Exp_s\\SB{3\\P{W_t - W_s}^2W_s} + \\Exp_s\\SB{3\\P{W_t-W_s}W_s} + W_s^3\\\\\n",
    "&= W_s^3 + 3W_s\\Exp\\SB{\\P{W_t-W_s}^2}\\\\\n",
    "&= W_s^3 + 3W_s\\P{t-s} \\neq W_s^3\n",
    "\\end{align}$$\n",
    "\n",
    "$\\P{2}$\n",
    "\n",
    "$\\bspace$Still let $X_t = X_t$, then\n",
    "\n",
    "$$\\begin{align}\n",
    "\\dd Y_t &= \\dd\\P{\\exp\\CB{-\\ffrac{1}{2}\\sigma^2 t} e^{\\sigma W_t}}\\\\\n",
    "&= Y_t\\P{-\\ffrac{1}{2}\\sigma^2 \\dd t - \\ffrac{1}{2}\\sigma^2 \\dd t + \\sigma\\dd W_t + \\ffrac{1}{2}\\sigma^2 \\dd t}\\\\\n",
    "&= Y_t\\P{-\\ffrac{1}{2}\\sigma^2 \\dd t + \\sigma \\dd W_t}\n",
    "\\end{align}$$\n",
    "\n",
    "$\\bspace$It's a martingale. We denote $M_t = \\exp\\CB{\\sigma W_t - \\ffrac{1} {2} \\sigma^2 t}$. For the expectation part:\n",
    "\n",
    "$$\\Exp\\SB{\\abs{M_t}} = \\int_{-\\infty}^{\\infty} \\exp\\CB{\\sigma W_t - \\ffrac{1} {2} \\sigma^2 t} \\cdot\\ffrac{1} {\\sqrt{2\\pi t}} \\exp\\CB{-\\ffrac{x^2} {2t}}\\dd{x} = 1 < \\infty$$\n",
    "\n",
    "$$\\Exp_s\\SB{M_t} = \\Exp_s\\SB{M_s\\cdot M_{t-s}} = M_s\\Exp_s\\SB{M_{t-s}} = M_s$$"
   ]
  },
  {
   "cell_type": "markdown",
   "metadata": {},
   "source": [
    "## Question 9\n",
    "\n",
    "$\\bspace$Here let $X_t = \\alpha W_t$ and we obtain\n",
    "\n",
    "$$\\begin{align}\n",
    "\\dd Z_t &= \\dd\\P{e^{X_t}}\\\\\n",
    "&= \\P{0 + 0 + \\ffrac{1}{2}\\alpha^2 e^{X_t}}\\dd t + \\alpha e^{X_t} \\dd W_t\\\\\n",
    "&= Z_t\\P{\\ffrac{1}{2}\\alpha^2 \\dd t + \\alpha \\dd W_t}\n",
    "\\end{align}$$\n",
    "\n",
    "$$\\begin{align}\n",
    "m\\P{t} &= \\Exp\\SB{Z_t} = \\Exp\\SB{e^{\\alpha W_t}}\\\\\n",
    "&= \\Exp\\SB{e^{\\alpha W_0} + \\int_0^t \\alpha e^{\\alpha W_s}\\;\\dd W_s + \\int_0^t\\ffrac{1}{2}\\alpha^2 e^{\\alpha W_s}\\;\\dd s}\\\\\n",
    "&= \\Exp\\SB{1} + \\Exp\\SB{\\int_0^t \\alpha e^{\\alpha W_s}\\;\\dd W_s} + \\Exp\\SB{\\int_0^t\\ffrac{1}{2}\\alpha^2 e^{\\alpha W_s}\\;\\dd s}\\\\\n",
    "&= 1 + 0 + \\int_0^t\\ffrac{1}{2}\\alpha^2 \\Exp\\SB{e^{\\alpha W_s}}\\;\\dd s\\\\\n",
    "&= 1 + \\ffrac{1}{2}\\alpha^2\\int_0^tm\\P{s}\\;\\dd s\n",
    "\\end{align}$$\n",
    "\n",
    "$$\\begin{align}\\dd m\\P{t} &= \\ffrac{1}{2}\\alpha^2 m\\P{t} + C\\\\\n",
    "\\Longrightarrow m\\P{t} &= \\exp\\CB{\\ffrac{1}{2}\\alpha^2 t}-\\ffrac{2C}{\\alpha^2}\\\\\n",
    "m\\P{0}=1\\Rightarrow m\\P{t} &= \\Exp\\SB{e^{\\alpha W_t}} = \\exp\\CB{\\ffrac{1}{2}\\alpha^2 t}\n",
    "\\end{align}$$"
   ]
  },
  {
   "cell_type": "markdown",
   "metadata": {},
   "source": [
    "## Question 10\n",
    "\n",
    "$\\bspace$To verify, we first rewrite the equation to $e^{\\alpha t}\\dd X_t = -\\alpha e^{\\alpha t}X_t\\dd t + e^{\\alpha t}\\dd W_t$ and this is equivalent to\n",
    "\n",
    "$$\\dd\\P{e^{\\alpha t}X_t} = e^{\\alpha t}\\dd W_t \\\\\n",
    "\\Longrightarrow e^{\\alpha t}X_t - 1 \\cdot X_0 = \\int_0^t e^{\\alpha s}\\;\\dd W_s\\\\\n",
    "\\Longrightarrow X_t = e^{-\\alpha t}x + e^{-\\alpha t}\\int_0^t e^{\\alpha s}\\;\\dd W_s\n",
    "$$\n",
    "\n",
    "$\\bspace$And about the mean\n",
    "\n",
    "$$\\begin{align}\n",
    "\\Exp\\SB{X_t} &= \\Exp\\SB{e^{-\\alpha t}x + e^{-\\alpha t}\\int_0^t e^{\\alpha s}\\;\\dd W_s}\\\\\n",
    "&= e^{-\\alpha t}x + e^{-\\alpha t}\\Exp\\SB{\\int_0^t e^{\\alpha s}\\;\\dd W_s}\\\\\n",
    "&= e^{-\\alpha t}x + e^{-\\alpha t} \\cdot 0\\\\\n",
    "&= e^{-\\alpha t}\n",
    "\\end{align}$$\n",
    "\n",
    "$\\bspace$To find the variance, by $\\Var{X_t}=\\Exp\\SB{X_t^2}-\\P{\\Exp\\SB{X_t}}^2$, we first need to apply the Itô's isommetry to find the second moment\n",
    "\n",
    "$$\\begin{align}\n",
    "\\Exp\\SB{X_t^2} &= \\Exp\\SB{e^{-2\\alpha t}x^2 + 2e^{-2\\alpha t}x\\int_0^t e^{\\alpha s}\\;\\dd W_s + e^{-2\\alpha t}\\P{\\int_0^t e^{\\alpha s}\\;\\dd W_s}^2}\\\\\n",
    "&= \\Exp\\SB{e^{-2\\alpha t}x^2} + \\Exp\\SB{ 2e^{-2\\alpha t}x\\int_0^t e^{\\alpha s}\\;\\dd W_s} + e^{-2\\alpha t}\\Exp\\SB{\\P{\\int_0^t e^{\\alpha s}\\;\\dd W_s}^2}\\\\\n",
    "&= e^{-2\\alpha t}x^2 + 0 + e^{-2\\alpha t}\\int_0^t \\Exp\\SB{e^{2\\alpha s}}\\dd s\\\\\n",
    "&= e^{-2\\alpha t}x^2 + \\ffrac{1}{2\\alpha}\\P{1 - e^{-2\\alpha t}}\n",
    "\\end{align}$$\n",
    "\n",
    "$\\bspace$With this, we can compute the final variance\n",
    "\n",
    "$$\n",
    "\\begin{align}\n",
    "\\Var{X_t}&=\\Exp\\SB{X_t^2}-\\P{\\Exp\\SB{X_t}}^2\\\\\n",
    "&= e^{-2\\alpha t}x^2 + \\ffrac{1}{2\\alpha}\\P{1 - e^{-2\\alpha t}} - x^2e^{-2\\alpha t}\\\\\n",
    "&= \\ffrac{1}{2\\alpha}\\P{1-e^{-2\\alpha t}}\n",
    "\\end{align}\n",
    "$$"
   ]
  },
  {
   "cell_type": "markdown",
   "metadata": {},
   "source": [
    "## Question 11\n",
    "\n",
    "$\\bspace$To make this simple, we write $\\dd X_t = \\mu \\dd t + \\sigma_t \\dd W_t$ where $W_t$ is the standard Brownian motion under measure $\\PP$. Let $\\widetilde W_t$ is that under measure $\\PP^*$, then we have\n",
    "\n",
    "$$\\dd X_t = \\nu \\dd t + \\sigma_t \\dd \\widetilde W_t$$\n",
    "\n",
    "$\\bspace$So we can define $\\widetilde W_t = W_t + \\ffrac{\\mu - \\nu}{\\sigma}t$. Then by Girsanov’s Theorem, we can define the measure $\\PP^*$\n",
    "\n",
    "$$\\left.\\ffrac{\\dd \\PP^*}{\\dd \\PP}\\right|_{\\FcF_t} = \\exp\\CB{-\\theta W_t - \\ffrac{1}{2}\\theta^2 t},\\bspace \\theta = \\ffrac{\\mu - \\nu}{\\sigma}$$"
   ]
  },
  {
   "cell_type": "markdown",
   "metadata": {},
   "source": [
    "## Question 12\n",
    "\n",
    "$\\bspace$By F-K formula, we have the solution of the corresponding stochastic differential equation\n",
    "\n",
    "$$\\dd X_t = \\mu_t\\dd t + \\sigma_t \\dd W_t$$\n",
    "\n",
    "$\\bspace$where $\\mu_t = 0$, $r = 0$, and $\\sigma_t = \\sigma$. So that the solution is, in integral form,\n",
    "\n",
    "$$X_t = \\sigma W_t + X_0$$\n",
    "\n",
    "$\\bspace$So that the solution $F\\P{t,x}$\n",
    "\n",
    "$$\\begin{align}\n",
    "F\\P{t,x} &= \\Exp\\SB{e^{-r\\P{T-t}} e^{X_T} \\mid X_t = x} \\\\\n",
    "&= \\Exp\\SB{e^{-0\\P{T-t}} e^{\\sigma W_T} \\mid W_t = x} \\\\\n",
    "&= \\Exp\\SB{e^{\\sigma\\P{ W_T - W_t +x}} \\mid W_t = x}\\\\\n",
    "&= e^{\\sigma x}\\Exp\\SB{e^{\\sigma\\P{ W_T - W_t}}}\\\\\n",
    "&= \\exp\\CB{\\sigma x + \\ffrac{\\sigma^2}{2}\\P{T-t}}\n",
    "\\end{align}$$"
   ]
  },
  {
   "cell_type": "markdown",
   "metadata": {},
   "source": [
    "***"
   ]
  }
 ],
 "metadata": {
  "kernelspec": {
   "display_name": "Python 3",
   "language": "python",
   "name": "python3"
  },
  "language_info": {
   "codemirror_mode": {
    "name": "ipython",
    "version": 3
   },
   "file_extension": ".py",
   "mimetype": "text/x-python",
   "name": "python",
   "nbconvert_exporter": "python",
   "pygments_lexer": "ipython3",
   "version": "3.5.2"
  },
  "toc": {
   "colors": {
    "hover_highlight": "#DAA520",
    "navigate_num": "#000000",
    "navigate_text": "#333333",
    "running_highlight": "#FF0000",
    "selected_highlight": "#FFD700",
    "sidebar_border": "#EEEEEE",
    "wrapper_background": "#FFFFFF"
   },
   "moveMenuLeft": true,
   "nav_menu": {
    "height": "12px",
    "width": "252px"
   },
   "navigate_menu": true,
   "number_sections": true,
   "sideBar": true,
   "threshold": 4,
   "toc_cell": false,
   "toc_section_display": "block",
   "toc_window_display": false,
   "widenNotebook": false
  }
 },
 "nbformat": 4,
 "nbformat_minor": 2
}
