{
 "cells": [
  {
   "cell_type": "markdown",
   "metadata": {},
   "source": [
    "# <center>Applied Stochastic Processes HW02</center>\n",
    "\n",
    "<center>**11510691 ç¨‹è¿œ$\\DeclareMathOperator*{\\argmin}{argmin}\n",
    "\\newcommand{\\using}[1]{\\stackrel{\\mathrm{#1}}{=}}\n",
    "\\newcommand{\\ffrac}{\\displaystyle \\frac}\n",
    "\\newcommand{\\space}{\\text{ }}\n",
    "\\newcommand{\\bspace}{\\;\\;\\;\\;}\n",
    "\\newcommand{\\QQQ}{\\boxed{?\\:}}\n",
    "\\newcommand{\\CB}[1]{\\left\\{ #1 \\right\\}}\n",
    "\\newcommand{\\SB}[1]{\\left[ #1 \\right]}\n",
    "\\newcommand{\\P}[1]{\\left( #1 \\right)}\n",
    "\\newcommand{\\dd}{\\mathrm{d}}\n",
    "\\newcommand{\\Tran}[1]{{#1}^{\\mathrm{T}}}\n",
    "\\newcommand{\\d}[1]{\\displaystyle{#1}}\n",
    "\\newcommand{\\EE}[2][\\,\\!]{\\mathbb{E}_{#1}\\left[#2\\right]}\n",
    "\\newcommand{\\Var}[2][\\,\\!]{\\mathrm{Var}_{#1}\\left[#2\\right]}\n",
    "\\newcommand{\\Cov}[2][\\,\\!]{\\mathrm{Cov}_{#1}\\left(#2\\right)}\n",
    "\\newcommand{\\Corr}[2][\\,\\!]{\\mathrm{Corr}_{#1}\\left(#2\\right)}\n",
    "\\newcommand{\\I}[1]{\\mathrm{I}\\left( #1 \\right)}\n",
    "\\newcommand{\\N}[1]{\\mathrm{N} \\left( #1 \\right)}\n",
    "\\newcommand{\\ow}{\\text{otherwise}}$æ˜Ÿ**</center>"
   ]
  },
  {
   "cell_type": "markdown",
   "metadata": {},
   "source": [
    "## Question 1\n",
    "\n",
    "$\\bspace \\begin{align}\n",
    "\\EE{X \\mid X > 1} &= \\int_{0}^{\\infty} x \\cdot f_X\\P{x \\mid X > 1} \\;\\dd{x} \\\\\n",
    "&= \\int_{1}^{\\infty} x \\cdot \\lambda e^{-\\lambda x} \\;\\dd{x} \\\\\n",
    "&= \\left.-\\P{x + \\ffrac{1} {\\lambda}}e^{-\\lambda x}\\right|_{1}^{\\infty} = \\P{1 + \\ffrac{1} {\\lambda}}e^{-\\lambda}\n",
    "\\end{align}$"
   ]
  },
  {
   "cell_type": "markdown",
   "metadata": {},
   "source": [
    "## Question 2\n",
    "\n",
    "$\\P{\\text a}$ \n",
    "\n",
    "$\\bspace \\begin{align}\n",
    "f_Y\\P{y} &= \\int_{-\\infty}^{\\infty} f\\P{x,y} \\;\\dd{x} \\\\\n",
    "&= \\int_{0}^{\\infty} \\ffrac{e^{-x/y} e^{-y}} {y} \\;\\dd{x} \\\\\n",
    "&= \\ffrac{1} {y} e^{-y} \\cdot \\left. \\P{-y\\exp\\P{-\\ffrac{1} {y}x}}\\right|_{0}^{\\infty} \\\\\n",
    "&\\using{y>0} \\ffrac{1} {y} e^{-y} \\cdot y = e^{-y}, y > 0\n",
    "\\end{align}$\n",
    "\n",
    "$\\bspace$ and $f_Y\\P{y} = 0$ otherwise.\n",
    "\n",
    "\n",
    "$\\P{\\text b}$ \n",
    "\n",
    "$\\bspace \\begin{align}\n",
    "\\EE{X \\mid Y = y} &= \\int_{-\\infty}^{\\infty} x \\cdot f_X\\P{x \\mid Y = y}\\;\\dd{x} \\\\\n",
    "&= \\int_{0}^{\\infty} x \\cdot \\ffrac{f_{X,Y}\\P{x,y}} {f_Y\\P{y}}\\;\\dd{x} \\\\\n",
    "&= \\int_{0}^{\\infty} x \\cdot \\ffrac{e^{-x/y} e^{-y}} {y} \\cdot {e^{y}}\\;\\dd{x} \\\\\n",
    "&= \\left.-\\P{x+y} \\exp\\P{-\\ffrac{1} {y} x}\\right|_{0}^{\\infty} \\using{y>0} y\n",
    "\\end{align}$\n",
    "\n",
    "$\\P{\\text C}$ \n",
    "\n",
    "$\\bspace \\begin{align}\n",
    "\\EE{X} &= \\EE{\\EE{X\\mid Y}} \\\\\n",
    "&= \\EE{Y} \\\\\n",
    "&= \\int_{-\\infty}^{\\infty} y\\cdot f_Y\\P{y} \\;\\dd{y} \\\\\n",
    "&= \\int_{0}^{\\infty} y \\cdot e^{-y} \\;\\dd{y} \\\\\n",
    "&= \\Big.-\\P{y+1}e^{-y}\\Big|_{0}^{\\infty} = 1\n",
    "\\end{align}$\n",
    "\n",
    "$\\bspace$ And to calculate its variance we first condition $X^2$ on $Y$, giving:\n",
    "\n",
    "$\\bspace \\begin{align}\n",
    "\\EE{X^2 \\mid Y = y} &= \\int_{0}^{\\infty} x^2 \\cdot \\ffrac{e^{-x/y} e^{-y}} {y} \\cdot {e^{y}}\\;\\dd{x} \\\\\n",
    "&= \\left.-\\P{x^2+2yx + 2y^2} \\exp\\P{-\\ffrac{1} {y} x}\\right|_{0}^{\\infty} \\using{y>0} 2y^2\n",
    "\\end{align}$\n",
    "\n",
    "Thus we can compute $\\EE{X^2}$ like:\n",
    "\n",
    "$\\bspace \\begin{align}\n",
    "\\EE{X^2} &= \\EE{\\EE{X^2\\mid Y}} \\\\\n",
    "&= \\EE{2Y^2} \\\\\n",
    "&= \\int_{-\\infty}^{\\infty} 2y^2\\cdot f_Y\\P{y} \\;\\dd{y} \\\\\n",
    "&= 2 \\int_{0}^{\\infty} y^2 \\cdot e^{-y} \\;\\dd{y} \\\\\n",
    "&= \\Big.-\\P{2y^2+ 4y + 4}e^{-y}\\Big|_{0}^{\\infty} = 4\n",
    "\\end{align}$\n",
    "\n",
    "$\\bspace \\Var{X} = \\EE{X^2} - \\P{\\EE{X}}^2 = 4 - 1^2 = 3$"
   ]
  },
  {
   "cell_type": "markdown",
   "metadata": {},
   "source": [
    "## Question 3\n",
    "\n",
    "$\\bspace \\begin{align}\n",
    "\\text{RHS} &= \\Big(\\EE{\\EE{\\P{X - \\EE{X \\mid Y}}^2 \\mid Y}}\\Big) + \\Big(\\EE{\\P{\\EE{X \\mid Y}}^2} - \\P{\\EE{\\EE{X \\mid Y}}}^2 \\Big) \\\\\n",
    "&= \\EE{\\P{X - \\EE{X \\mid Y}}^2} + \\EE{\\P{\\EE{X \\mid Y}}^2} - \\P{\\EE{X}}^2 \\\\\n",
    "&= \\EE{X^2} - 2\\cdot \\EE{X \\cdot \\EE{X \\mid Y}} + 2 \\cdot \\EE{\\P{\\EE{X \\mid Y}}^2} - \\P{\\EE{X}}^2 \\\\\n",
    "&= \\EE{X^2} - \\P{\\EE{X}}^2 - 2 \\cdot \\EE{\\EE{X \\cdot \\EE{X \\mid Y} \\mid Y}}+ 2 \\cdot \\EE{\\P{\\EE{X \\mid Y}}^2} \\\\\n",
    "&= \\Var{X} - 2 \\cdot \\EE{\\P{\\EE{X \\mid Y}}^2} + 2 \\cdot \\EE{\\P{\\EE{X \\mid Y}}^2} = \\Var{X} = \\text{LHS}\n",
    "\\end{align}$"
   ]
  },
  {
   "cell_type": "markdown",
   "metadata": {},
   "source": [
    "## Question 4\n",
    "\n",
    "$\\P{\\text a}$\n",
    "\n",
    "$\\bspace \\begin{align}\n",
    "X &= \\sum_{i=1}^{N}T_i\n",
    "\\end{align}$\n",
    "\n",
    "$\\P{\\text b}$\n",
    "\n",
    "$\\bspace$ To find $\\EE{N}$ we condition that on $Y$, the first choice:\n",
    "\n",
    "$\\bspace \\begin{align}\n",
    "\\EE{N} &= \\EE{N \\mid Y = 1} \\cdot P\\CB{Y = 1} + \\EE{N \\mid Y = 2} \\cdot P\\CB{Y = 2} + \\EE{N \\mid Y = 3} \\cdot P\\CB{Y = 3} \\\\\n",
    "&= \\ffrac{1} {3} \\P{1 + 1 + \\EE{N} + 1 + \\EE{N}}\n",
    "\\end{align}$\n",
    "\n",
    "$\\bspace$ Then we solve the preceding equation and find the solution that tis $\\EE{N} = 3$\n",
    "\n",
    "$\\P{\\text c}$\n",
    "\n",
    "$\\bspace$ Since $N$ is the total number of choices, or equivalently, there's no $N+1$ choice. Thus $T_N \\equiv 2$ and $\\EE{T_N} = 2$.\n",
    "\n",
    "$\\P{\\text d}$\n",
    "\n",
    "$\\bspace \\begin{align}\n",
    "\\EE{\\sum_{i=1}^{N}T_i \\mid N = n} &= \\EE{\\sum_{i=1}^{n-1}T_i \\mid N = n} + \\EE{T_n \\mid N = n} \\\\\n",
    "&= \\EE{\\sum_{i=1}^{n-1}T_i} + \\EE{T_n} \\\\\n",
    "&= \\P{n-1} \\cdot \\ffrac{1} {2} \\P{3+5} + 2 = 4n - 2\n",
    "\\end{align}$\n",
    "\n",
    "$\\P{\\text e}$ \n",
    "\n",
    "$\\bspace \\begin{align}\n",
    "\\EE{X} &= \\EE{\\EE{\\sum_{i=1}^{N}T_i \\mid N} } \\\\\n",
    "&= \\EE{4N - 2} \\\\\n",
    "&= 4\\cdot \\EE{N} - 2 = 4 \\times 3 - 2 = 10\n",
    "\\end{align}$"
   ]
  },
  {
   "cell_type": "markdown",
   "metadata": {},
   "source": [
    "## Question 5\n",
    "\n",
    "$\\P{\\text a}$\n",
    "\n",
    "$\\bspace \\begin{align}\n",
    "\\EE{X_1} = 1 \\times \\ffrac{r} {r+b} + 0 \\times \\ffrac{b} {r+b} = \\ffrac{r} {r+b}\n",
    "\\end{align}$\n",
    "\n",
    "$\\P{\\text b}$\n",
    "\n",
    "$\\bspace$ First we let $Y_i = 1$ if the $i\\texttt{-th}$ draw is a red one and $0$ otherwise.\n",
    "\n",
    "$\\bspace \\begin{align}\n",
    "\\EE{X_2} &= \\EE{X_2 \\mid Y_1 = 1} \\cdot P\\CB{Y_1 = 1} + \\EE{X_2 \\mid Y_1 = 0} \\cdot P\\CB{Y_1 = 0} \\\\\n",
    "&= \\P{2\\times \\ffrac{r+m} {r+b+m} \\times \\ffrac{r} {r+b} + \\ffrac{b} {r+b + m} \\cdot \\ffrac{r} {r+b}} + \\ffrac{r} {r+b + m} \\cdot \\ffrac{b} {r+b} = \\ffrac{2r} {r+b}\n",
    "\\end{align}$\n",
    "\n",
    "$\\P{\\text c}$\n",
    "\n",
    "$\\bspace \\begin{align}\n",
    "\\EE{X_3} &= \\EE{\\EE{\\EE{X_3 \\mid Y_2}}\\mid Y_1} \\\\\n",
    "&= \\EE{ \\EE{X_3 \\mid Y_2 = 1}\\cdot P\\CB{Y_2 = 1} + \\EE{X_3 \\mid Y_2 = 0}\\cdot P\\CB{Y_2 = 0}\\mid Y_1} \\\\\n",
    "&= \\EE{X_3 \\mid Y_2 = 1, Y_1 = 1} \\cdot P\\CB{Y_2 = 1 \\mid Y_1 = 1} \\cdot P\\CB{Y_1 = 1} \\\\\n",
    "&\\bspace + \\EE{X_3 \\mid Y_2 = 1, Y_1 = 0} \\cdot P\\CB{Y_2 = 1 \\mid Y_1 = 0} \\cdot P\\CB{Y_1 = 0} \\\\\n",
    "&\\bspace + \\EE{X_3 \\mid Y_2 = 0, Y_1 = 1} \\cdot P\\CB{Y_2 = 0 \\mid Y_1 = 1} \\cdot P\\CB{Y_1 = 1} \\\\\n",
    "&\\bspace + \\EE{X_3 \\mid Y_2 = 0, Y_1 = 0} \\cdot P\\CB{Y_2 = 0 \\mid Y_1 = 0} \\cdot P\\CB{Y_1 = 0} \\\\\n",
    "&= \\P{3 \\times \\ffrac{r+2m} {r+b+2m} + 2 \\times \\ffrac{b} {r+b+2m}}\\cdot \\ffrac{r+m} {r+b+m} \\cdot \\ffrac{r} {r+b} \\\\\n",
    "&\\bspace + \\P{2\\times\\ffrac{r+m} {r+b+2m} + \\ffrac{b+m} {r+b+2m}} \\cdot \\ffrac{r} {r+b+m} \\cdot \\ffrac{b} {r+b} \\\\\n",
    "&\\bspace + \\P{2\\times\\ffrac{r+m} {r+b+2m} + \\ffrac{b+m} {r+b+2m}} \\cdot \\ffrac{b} {r+b+m} \\cdot \\ffrac{r} {r+b} \\\\\n",
    "&\\bspace + \\ffrac{r} {r+b+2m} \\cdot \\ffrac{b+m} {r+b+m} \\cdot \\ffrac{b} {r+b} \\\\\n",
    "&= \\ffrac{3r} {r+b}\n",
    "\\end{align}$\n",
    "\n",
    "$\\P{\\text d}$\n",
    "\n",
    "$\\bspace$ Based on the preceding results, I conjecture that $\\EE{X_k} = \\ffrac{kr} {r+b}$ for $k = 1, 2, \\dots$. To prove this we first let $r_i$ and $b_i$ denote the number of red balls and blue balls at $i\\texttt{-th}$ draw. Then $r_1 = r$ and $b_1 = b$; by induction, we let this equation holds for $k =1,2,\\dots,n-1$ and we condtion $X_n$ on $Y_{n-1}$ finding that:\n",
    "\n",
    "$\\bspace \\begin{align}\n",
    "\\EE{X_n} &= \\EE{\\EE{X_n \\mid Y_{n-1}}} \\\\\n",
    "&= \\EE{X_n \\mid Y_{n-1} = 1} \\cdot P\\CB{Y_{n-1} = 1} + \\EE{X_n \\mid Y_{n-1} = 0} \\cdot P\\CB{Y_{n-1} = 0} \\\\\n",
    "&= \\P{\\P{2 + \\ffrac{\\P{k-2}r} {r+b}}\\cdot\\ffrac{r_{n-1} + m} {r_{n-1} + b_{n-1} + m} + \\P{1+\\ffrac{\\P{k-2}r} {r+b}} \\cdot \\ffrac{b_{n-1}} {r_{n-1} + b_{n-1} + m}} \\cdot \\ffrac{r_{n-1}} {r_{n-1} + b_{n-1}} \\\\\n",
    "&\\bspace + \\P{\\P{1+\\ffrac{\\P{k-2}r} {r+b}} \\cdot \\ffrac{r_{n-1}} {r_{n-1} + b_{n-1} + m} + \\ffrac{\\P{k-2}r} {r+b} \\cdot \\ffrac{b_{n-1} + m} {r_{n-1} + b_{n-1} + m}} \\cdot \\ffrac{b_{n-1}} {r_{n-1} + b_{n-1}} \\\\\n",
    "&= \\ffrac{nr} {r+b}\n",
    "\\end{align}$\n",
    "\n",
    "$\\bspace$ solved...ðŸ˜œðŸ˜œðŸ˜œ\n",
    "\n",
    "$\\P{\\text e}$\n",
    "\n",
    "$\\bspace$ To be intuitive, honestly, my first impression on this problem is:\n",
    "\n",
    "$$\\sum_{i=0}^{n} \\P{\\binom{n} {i} \\cdot i \\cdot \\ffrac{\\d{\\prod_{j=0}^{i-1}\\SB{r+jm}}\\d{\\prod_{j=0}^{n-i-1} \\SB{b+jm}}} {\\d{\\prod_{k=0}^{n-1}\\SB{r+b+km}}}}$$\n",
    "\n",
    "$\\bspace$ That's not something that's gonna help, so another thoughts, after $\\EE{Y_2}$ is given. Since $\\EE{Y_2} = \\EE{Y_1}$, maybe now the urn can be consider in the same \"state\" with before. So that $\\EE{Y_{n-1}} = \\EE{Y_n}$ will always hold and thus $\\EE{X_n} = \\sum_n \\EE{Y_i} = n\\ffrac{r} {r+b}$"
   ]
  },
  {
   "cell_type": "markdown",
   "metadata": {},
   "source": []
  }
 ],
 "metadata": {
  "kernelspec": {
   "display_name": "Python 3",
   "language": "python",
   "name": "python3"
  },
  "language_info": {
   "codemirror_mode": {
    "name": "ipython",
    "version": 3
   },
   "file_extension": ".py",
   "mimetype": "text/x-python",
   "name": "python",
   "nbconvert_exporter": "python",
   "pygments_lexer": "ipython3",
   "version": "3.5.2"
  }
 },
 "nbformat": 4,
 "nbformat_minor": 2
}
